\documentclass[14pt,fleqn]{extarticle}
\RequirePackage{prepwell-eng}
\previewoff
\begin{document}
\begin{problem}
\statement
	
%text
If $f(x) = x + 7$ and $g(x) = x-7, x\in\mathbb{R},$ 
then find $(f\circ g)(7)$
%
\begin{step}
	\begin{options}
		\correct

		\[(f\circ g)(x) = f\left( g\left( x\right)\right) \]

		\incorrect

		\[(f\circ g)(x) = f(x)\cdot g(x) \]

	\end{options}
	\reason

	%text
$(f\circ g)(x)$ is simply shorthand for $ f\left( g\left( x\right)\right)$.
And similarly $\left(g\circ f \right)(x) = g \left( f \left(x \right) \right)$\newline 

And note that $ f \left(g(x) \right)\neq g \left(f(x) \right)$
\end{step}
\begin{step}
	\begin{options}
		\correct

		\[\therefore (f\circ g)(7) = 7 \]

		\incorrect

		\[\therefore (f\circ g)(7) = 0\]

	\end{options}
	\reason

	\begin{align}
(f\circ g)(x) &= f\left( g\left( x \right) \right) = g(x) + 7 \\
&= (x-7) + 7 = x \\ 
\therefore (f\circ g)(7) &= 7
\end{align} 
\end{step}
\end{problem}
\end{document}
