

\question[3] Find an expression for the sum of the first $n$ terms of the series 
\[ 1^2 + (1^2+2^2) + (1^2+2^2+3^2) + \ldots \]

\begin{solution}[\halfpage]
  If $a_n$ be the $n-$th term in the series, then notice that 
  \[ a_n = \sum_{k=1}^n k^2 = \eSumOfSquares{n} \]
  But what we need is 
  \[ S_n = \sum_{k=1}^n a_k \]
  And therefore, 
	\begin{align}
		S_n &= \sum_{k=1}^n a_k = \sum_{k=1}^{n} \eSumOfSquares{k} \\
		&= \dfrac{1}{6}\cdot\sum_{k=1}^{n}(2k^3+3k^2+k) \\ 
    &= \dfrac{1}{6}\cdot\left[ 2\sum_{k=1}^{n} k^3 + 3\sum_{k=1}^{n} k^2 + \sum_{k=1}^{n} k \right] \\
		&= \dfrac{1}{6}\cdot\left[ 2\cdot\eSumOfCubes{n} + 3\cdot\eSumOfSquares{n} + \eSumOfN{n}\right] \\
		&= \dfrac{n\cdot(n+1)}{12}\cdot\left[ \underbrace{n\cdot(n+1) + 2n + 1 + 1}_{=(n+1)\cdot(n+2)}\right]\\
		&= \dfrac{n\cdot(n+1)^2\cdot(n+2)}{12}
	\end{align}
\end{solution}
\ifprintanswers\begin{codex}$\dfrac{n\cdot (n+1)^2\cdot (n+2)}{12}$\end{codex}\fi
