\documentclass[14pt,fleqn]{extarticle}
\RequirePackage{prepwell-eng}

\newcommand\msq{\left(1-x^2 \right)}
\newcommand\psq{\left(1+x^2 \right)}

\previewoff 

\begin{document} 
\begin{problem}
	\statement 
    
    If $y = \dfrac{2x}{1-x^2}$, then find $\dfrac{d}{dx}y$ 
    
    \begin{step}
  \begin{options} 
       
     \incorrect
     
     \begin{align}
	\text{Let } x &= \sin\phi \implies dx = \cos\phi\cdot d \phi \\
	\text{and } y &= \sin 2\phi \\
	\therefore \ddx y &= \underbrace{\frac{d}{d\phi} y \cdot \ddx \phi}_{\text{Chain Rule}} = (2\cos2\phi)\cdot \ddx \phi
\end{align}
    \end{options} 
     \reason 
     
     $x=\sin\phi$ is the wrong substitution to make \newline 
     
     Instead, try $x = \tan\phi$ 
     \begin{align}
     x &= \tan\phi \implies dx = \sec^2\phi\cdot d\phi \\
     \text{and } y &= \frac{2\tan\phi}{1-\tan^2\phi} = \tan 2\phi \\
     \therefore \ddx y &= \underbrace{\frac{d}{d\phi}y\cdot \ddx \phi}_{\text{Chain Rule}} = (2\sec^2 2\phi)\cdot \ddx\phi 
\end{align}
       
\end{step} 

\begin{step}
  \begin{options} 
     \correct 

\begin{align}
	\ddx y &= 2\cdot \dfrac{\sec^2 2\phi}{\sec^2\phi} \\
	\therefore \ddx y &= 2 \left[\dfrac{\psq}{\msq^2} \right]
\end{align}       

     \incorrect

\begin{align}
	\ddx y &= 2\cdot \dfrac{\sec^2 2\phi}{\sec^2\phi} \\
	\therefore \ddx y &= 2 \left[\dfrac{\msq^2}{\psq} \right]
\end{align}
        
    \end{options} 
     \reason 
       
     \begin{align}
	\ddx y &= \underbrace{2 \sec^2 2\phi \cdot \ddx \phi = \frac{2\sec^2 2\phi}{\sec^2\phi}}_{\text{Recall that } dx = \sec^2\phi\cdot d\phi}  \\
	&= \underbrace{2 \left[\dfrac{1 + \tan^2 2\phi}{1+\tan^2\phi} \right]}_{\sec^2\theta = 1 + \tan^2\theta} \\
	&= 2 \left[\dfrac{1 + \left(\frac{2\tan\phi}{1-\tan^2\phi} \right)^2}{1 + \tan^2\phi} \right] \\
	&= 2 \left[\dfrac{1 + \left(\frac{2x}{1-x^2} \right)^2}{1+x^2} \right] \\
	&= 2 \left[\dfrac{\left(1-x^2 \right)^2 + 4x^2}{\left(1-x^2 \right)^2\cdot \left(1+x^2 \right)} \right] \\
	&= 2 \left[\dfrac{x^4 + 2x^2 + 1}{\left(1-x^2 \right)^2\cdot \left(1+x^2 \right)} \right] \\
	&= 2 \left[\dfrac{\left(1+x^2 \right)^2}{\left(1-x^2 \right)^2\cdot \left(1+x^2 \right)} \right] \\
	&= 2 \left[\dfrac{\left(1+x^2 \right)}{\left(1-x^2 \right)^2} \right]
\end{align} 
\end{step}
\end{problem} 
\end{document} 
