
\question[3] Prove - or disprove - the following proposition using mathematical induction
\[ 1^2 + 3^2 + 5^2 + \cdots + (2n-1)^2 = \dfrac{1}{3}(4n^3-n) \]

\insertQR{}

\begin{solution}[\halfpage]
  \textbf{If} the proposition is true for all $n$, \textbf{then} the following should also 
  be true
  \begin{align}
    &\underbrace{1^2+3^2+5^2+\cdots+(2n-1)^2}_{\frac{1}{3}(4n^3-n)} +
    \lbrace 2\cdot(n+1)-1\rbrace^2 = \dfrac{1}{3}\left[4\cdot(n+1)^3-(n+1) \right] \\
    &\implies \dfrac{1}{3}\left[ (4n^3-n) + 3\cdot\underbrace{(4n^2+4n+1)}_{(2n+1)^2} \right] = 
    \dfrac{1}{3}\left[ 4\cdot (n^3+3n^2+3n+1) - n - 1\right] \\
    &\dfrac{1}{3}\left[ 4n^3-n +12n^2+12n+3\right] =
    \dfrac{1}{3}\left[ 4n^3 + 12n^2 + 12n + 4 -n - 1\right] \\
    &\dfrac{1}{3}\left[ 4n^3+12n^2+11n + 3\right] = \dfrac{1}{3}\left[ 4n^3 + 12n^2 +11n + 3\right]
  \end{align}

  What we have proven is that if the proposition is true for $n$, then it is also 
  true for $n+1$. 

  Also, note that the proposition is true for $n=1\implies$ it is also true for $n=2, n=3$ 
  and so on. Hence proved.
\end{solution}

