\documentclass[14pt,fleqn]{extarticle}
\RequirePackage{prepwell-eng}

\previewoff

\begin{document}

\begin{skill}
\begin{narrow}

\textcolor{blue}{Inverse Trigonometry (Inversion)}

\small\textbf{Example }  $\sin^{-1} \left(\sin\theta \right) \text{ \& }\sin \left(\sin^{-1} x \right)$

\end{narrow}
\reason 

%text
Remember \[ \qquad \sin^{-1} (\sin x) \neq \dfrac{1}{\sin}\cdot \sin x\]

Similarly \[ \qquad \cos\left( \cos^{-1}x \right) \neq \cos\cdot\dfrac{1}{\cos} x\]

The above statements are meaningless\newline 

The ones below are however true -- and
follow \underline{straight from the definition}\newline 

%
\begin{tabular}{MMM} 
\midrule 
\textbf{If} & \textbf{Then} & \textbf{Also} \\ 
\midrule 
\sin\theta = x & \sin^{-1}(\sin \theta) = \theta & \sin(\sin^{-1}x) = x \\ 
\midrule 
\cos\theta = x & \cos^{-1}(\cos \theta) = \theta & \cos(\cos^{-1}x) = x \\ 
\midrule 
\tan\theta = x & \tan^{-1}(\tan \theta) = \theta & \tan(\tan^{-1}x) = x \\ 
\midrule 
\csc\theta = x & \csc^{-1}(\csc\theta) = \theta & \csc(\csc^{-1}x) = x \\ 
\midrule 
\sec\theta = x & \sec^{-1}(\sec \theta) = \theta & \sec(\sec^{-1}x) = x \\ 
\midrule 
\cot\theta = x & \cot^{-1}(\cot \theta) = \theta & \cot(\cot^{-1}x) = x \\ 
\midrule
\end{tabular}
\end{skill}
\end{document}
