
\ifnumequal{\value{rolldice}}{0}{
}{
  \ifnumequal{\value{rolldice}}{1}{
  }{
    \ifnumequal{\value{rolldice}}{2}{
    }{
    }
  }
}

\question[5] Find $f(x)$ such that,
    \[\int \left(\dfrac{\tan^{-1}x}{x}-\dfrac{\ln x}{1+x^2}\right)\dfrac{1}{(\tan^{-1}x)^2}dx = \dfrac{f(x)}{\tan^{-1}x}+C\]

\begin{solution}[\fullpage]
  \begin{align}
    I &= \int \left(\dfrac{\tan^{-1}x}{x}-\dfrac{\ln x}{1+x^2}\right)\dfrac{1}{(\tan^{-1}x)^2}dx \\
      &= \int \left(\dfrac{\tan^{-1}x}{x}\cdot\dfrac{1}{(\tan^{-1}x)^2}-
                    \dfrac{\ln x}{1+x^2}\cdot\dfrac{1}{(\tan^{-1}x)^2}\right)dx \\
      &= \int \left(\dfrac{1}{x\tan^{-1}x}-\dfrac{\ln x}{(1+x^2)(\tan^{-1}x)^2}\right)dx \\
      &= \int \left(\dfrac{1+x^2}{x\tan^{-1}x}-\dfrac{\ln x}{(\tan^{-1}x)^2}\right)
              \cdot\dfrac{1}{1+x^2}dx \\
      &\text{Let}\quad x=\tan t\implies\tan^{-1}x=t\implies \dfrac{1}{1+x^2}dx=dt \nonumber \\
      &= \int \dfrac{1+\tan^2 t}{t\tan t}-\dfrac{\ln (\tan t)}{t^2}dt \\
      &= \underbrace{\int\dfrac{1+\tan^2 t}{t\tan t}dt}_{I_1}-
         \underbrace{\int\dfrac{\ln (\tan t)}{t^2}dt}_{I_2} \\
    I_2 &= \int\dfrac{\ln (\tan t)}{t^2}dt 
         = \int\underbrace{\dfrac{\ln (\tan t)}{1}}_{f_1}\cdot\underbrace{\dfrac{1}{t^2}}_{f_2}dt \\
        &\text{Using integration by parts} \nonumber \\
    I_2 &= \ln(\tan t)\cdot\dfrac{t^{-1}}{-1} - 
           \int \dfrac{1}{\tan t}\cdot\sec^{2}t\cdot\dfrac{t^{-1}}{-1}dt \\
        &= -\dfrac{\ln(\tan t)}{t} + C + \int \dfrac{\sec^{2}t}{t\tan t}dt \\
        &\text{Substitute back into equation in step (6)} \nonumber \\
    I &= \int\dfrac{1+\tan^2 t}{t\tan t}dt + \dfrac{\ln(\tan t)}{t} - \int \dfrac{\sec^{2}t}{t\tan t}dt + C \\
      &= \int\dfrac{\sec^2 t}{t\tan t}dt + \dfrac{\ln(\tan t)}{t} - \int \dfrac{\sec^{2}t}{t\tan t}dt + C \\
      &= \dfrac{\ln(\tan t)}{t} = \dfrac{\ln x}{\tan^{-1}x} + C
  \end{align}
  Therefore $f(x)=\ln x$
\end{solution}
\ifprintanswers\begin{codex}$f(x)=\ln x$\end{codex}\fi
