

\question[3] Find an expression for the sum of the first $n$ terms of the following series 
\[ 1^3 + 3^3 + 5^3 + 7^3 \ldots \]

\begin{solution}[\halfpage]
  If $a_n$ be the $n-$th term of the series, then 
  \[ a_n = (2n-1)^3,\, n\geq 1 \] 
	Hence, the sum of the first $n$ terms would be 
	\begin{align}
		S_n &= \sum_{k=1}^{n}(2k-1)^3 = \overbrace{\sum_{k=1}^n (8k^3 - 12k^2 + 6k - 1)}^{(a-b)^3 = a^3-3a^2b+3ab^2-b^3} \\
    &= 8\sum_{k=1}^{n}k^3 - 12 \sum_{k=1}^{n} k^2 + 6 \sum_{k=1}^{n} k - \sum_{k=1}^{n} 1 \\
		&= 8\cdot\eSumOfCubes{n} - 12\cdot\eSumOfSquares{n} \nonumber\\
    & + 6\cdot\eSumOfN{n} - n \\
		&= n\cdot(n+1)\cdot[2n\cdot(n+1) - 2\cdot(2n+1) + 3 ] - n \\
		&= n\cdot(n+1)\cdot(2n^2-2n+1) - n \\
    &= n\cdot\left[ (n+1)\cdot(2n^2-2n+1) - 1\right] \\
    &= n\cdot\left( 2n^3-2n^2+n + 2n^2-2n + 1 -1\right) \\
    &= n\cdot(2n^3-n) = n^2\cdot(2n^2-1)
	\end{align}
\end{solution}
 
\ifprintanswers\begin{codex}$n^2\cdot(2n^2-1)$\end{codex}\fi
