\documentclass[14pt,fleqn]{extarticle}
\RequirePackage{prepwell}

\previewoff 

\begin{document} 
\begin{snippet}
    \correct
    \[ \ddx \sin^{-1} \left(\cos x \right) = \ddx \left(\frac\pi{2} -x \right) = -1\]
    
    \reason
  
  If $f(x) = \sin^{-1} \left(\cos x \right)$, then note that 
  \begin{align}
	f(x) &= \underbrace{\sin^{-1} \left[\sin \left(\frac\pi{2}-x \right) \right] = \frac\pi{2}- x}_{\sin^{-1} \left(\sin\theta \right) = \theta} \\
	\therefore \ddx f(x) &= \ddx \left(\frac\pi{2}-x \right) = -1
\end{align}
\end{snippet} 
\end{document} 