
\question[4] Prove - or disprove - the following proposition
\[ x^n - y^n \text{ is divisible by } x - y,\, x\neq y\]

\insertQR{}

\begin{solution}
  It is easy to see that the proposition is true for $n=1$. So, let us assume 
  that it is true for some $n\neq 1\implies (x^n-y^n) = (x-y)\cdot Q(x,y)$ - where
  $(Q(x,y)$ is some polynomial is $x,y$.

  Also, $x = y + (x-y)$. Which means, that 
  \begin{align}
    \dfrac{x^{n+1}-y^{n+1}}{x-y} &= 
    \dfrac{(y+(x-y))\cdot x^n - y\cdot y^n}{x-y} \\
    &= x^n + y\cdot\underbrace{\left[ \dfrac{x^n-y^n}{x-y} \right]}_{=Q(x,y)}
  \end{align}

  What the last equation says is \textbf{ that if }, $x^n-y^n$ is a multiple of $x-y$,
  \textbf{ then so is} $x^{n+1}-y^{n+1}$.

  And given that the proposition is true for $n=1$, it must also be true 
  for $n=2,3,4,\ldots,\infty$. Hence proved.
\end{solution}

