\documentclass[14pt,fleqn]{extarticle}
\RequirePackage{prepwell}
\previewoff
\begin{document}

\newcommand\ea{1 + \sqrt{\tan x}}
\newcommand\eb{1 + \sqrt{\cot x}}
\newcommand\ec{\frac{\sqrt{\tan x}}{\ea}}
\newcommand\intg{\int_{\frac\pi{6}}^{\frac\pi{3}}}
\newcommand\etan{\sqrt{\tan x}}

Evaluate the following \[\qquad \int_\frac{\pi}{6}^\frac{\pi}{3}\dfrac{dx}{1+\sqrt{\tan x}}\]

\newcard

\[ A = \intg \frac{dx}{\ea} = \intg \frac{dx}{\eb}\]

\newcard 

There is a nice little rule that says 
\[ \quad \int_a^b f(x)\cdot dx = \int_a^b f \left(a+b-x \right)\cdot dx \] 

When applied to the given integral, we get 

\begin{align}
	A &= \intg \frac{dx}{\ea} = \intg \frac{dx}{1+\sqrt{\tan \left( \frac\pi{3}+\frac\pi{6} - x\right)}} \\
	&= \intg \frac{dx}{1 + \sqrt{\tan \left(\frac\pi{2} - x \right)}} = \intg \frac{dx}{1+\sqrt{\cot x}}
\end{align}

\newcard 

\[ A + A = \intg dx \implies A = \frac{\pi}{12}\]

\newcard 

\begin{align}
	A &= \intg \frac{dx}{\eb} = \intg \frac{dx}{1 + \frac{1}{\sqrt{\tan x}}} \\
	&= \intg \frac{\sqrt{\tan{x}}}{1+ \sqrt{\tan x}}\cdot dx  \\
	\text{Also } A &= \intg \frac{dx}{\ea} \\
	\therefore A + A &= \intg \left[ \frac{1}{1 + \etan} + \frac{\etan}{1 + \etan}\right]\cdot dx \\
	&= \intg \frac{1 + \etan}{1+\etan}\cdot dx = \intg dx \\
	\therefore 2A &= \left[x \right]_{\frac\pi{6}}^{\frac\pi{3}} = \left[\frac\pi{3} - \frac\pi{6} \right] = \frac\pi{6} \\
	\text{Hence } A &= \frac\pi{12}
\end{align}

\end{document}