
\question[4] Prove - or disprove - the following proposition using mathematical induction 
\[ x^{2n} - 1 \text{ is divisible by } x + 1,\, x\neq -1 \]

\insertQR{}

\begin{solution}[\halfpage]
  \textbf{Insight \#1: Meaning of divisibility of polynomials}

  If a polynomial $A(x)$ is divisible by another polynomial $B(x)$, then it means 
  \[ A(x) = B(x)\cdot C(x)\text{ where } C(x) = \text{ another polynomial in }x \] 
  We can see that the proposition is true for $n=1$
  \[ x^{2n} - 1 = \underbrace{x^2 - 1}_{A(x)} = \underbrace{(x+1)}_{B(x)}\cdot\underbrace{(x-1)}_{C(x)} \] 

  \textbf{Hence, if} $x^{2n}-1$ is divisible by $x+1$, that is 
  \[ x^{2n}-1 = P(x)\cdot (x+1) \] 
  
  then, 
  \begin{align}
    \dfrac{x^{2\cdot(n+1)}-1}{x+1} &= \overbrace{\dfrac{x^2\cdot x^{2n} - x^2 + x^2 - 1}{x+1}}^{\text{adding and subtracting $x^2$}} \\
    &= \underbrace{x^2\cdot\underbrace{\dfrac{(x^{2n} - 1)}{x+1}}_{P(x)} + \underbrace{x-1}_{\frac{x^2-1}{x+1}}}_{\text{Another polynomial}}
  \end{align}

  In short, we have shown that 
  \[ \dfrac{x^{2n}-1}{x+1} = P(x)\implies\dfrac{x^{2\cdot(n+1)}-1}{x+1} = x^2\cdot P(x) + (x-1) = Q(x) \]
  And as the proposition is true for $n=1$, it is also true for $n=2,3,4,\ldots\infty$.

\end{solution}
