

\question[3] Prove the following 
  \[\sin^8\theta - \cos^8\theta = (\sin^2\theta - \cos^2\theta)\cdot(1-2\sin^2\theta\cos^2\theta)\]


\ifprintanswers
\fi 

\begin{solution}[\halfpage]
   \begin{align}
      \underbrace{\sin^8\theta - \cos^8\theta}_{a^2-b^2} &= 
      \underbrace{(\sin^4\theta - \cos^4\theta)\cdot(\sin^4\theta + \cos^4\theta)}_{(a-b)\cdot(a+b)} \\
      &= (\sin^2\theta - \cos^2\theta)\cdot\underbrace{(\sin^2\theta + \cos^2\theta)}_{=1}\cdot
         \underbrace{(\sin^4\theta + \cos^4\theta)}_{a^2+b^2 = (a+b)^2 - 2ab} \\
      &= (\sin^2\theta - \cos^2\theta)\cdot\left[\underbrace{(\sin^2\theta + \cos^2\theta)^2}_{=1} -
         2\sin^2\theta\cos^2\theta\right] \\
      &= (\sin^2\theta - \cos^2\theta)\cdot(1-2\sin^2\theta\cos^2\theta)
   \end{align}
\end{solution}
