\documentclass[14pt,fleqn]{extarticle}
\RequirePackage{prepwell}
\previewoff
\begin{document}

\newcommand\xy{\frac{x}{y}}
\newcommand\yx{\frac{y}{x}}
\newcommand\ebz{e^{\frac{1}{z}}}
\newcommand\ez{e^z}


Solve the following differential equation 
\[ \quad 2y e^\xy\cdot dx + \left(y - 2xe^\xy \right)\cdot dy = 0 \]
and find the particular solution given that $x =0$ when $y=1$

\newcard 
%
\[ \frac{dy}{dx} = -\frac{2y\cdot e^\xy}{y - 2xe^\xy} = F \left(\frac{y}{x} \right)\]

Hence, the given equation is a \underline{homogenous} differential equation 

\newcard 

\[ \frac{dy}{dx} + \frac{2e^\xy}{y-2x e^\xy}\cdot y = 0 \]

This is of the form 
\[ \quad \frac{dy}{dx} + P(x)\cdot y = Q(x) \]
Hence, the given differential equation is a \underline{linear} differential equation

\newcard
\smallmath 
\begin{align}
	2y e^\xy\cdot dx &+ \left(y - 2xe^\xy \right)\cdot dy  = 0  \\
	\implies \left(y-2x e^\xy \right)\cdot dy  &= -2y e^\xy\cdot dx \\
	\text{or }\frac{dy}{dx} &= -\frac{2y\cdot e^\xy}{\left(y-2x\cdot e^\xy \right)} \\
	&= \underbrace{-\frac{2 \left(\yx \right)\cdot e^\xy}{\yx - 2\cdot e^\xy}}_{\text{Divide throughout by $x$}} \\
	&= F \left(\yx \right)
\end{align}

Hence, this is a \underline{homogenous} differential equation 

\newcard 


If $z = \dfrac{y}{x}$ then 
\begin{align}
	\frac{dy}{dx} &= z + x \frac{dz}{dx} = - \frac{2z\cdot \ebz}{z - 2\ebz} \\
	\implies -\frac{dx}{x} &= \left[\frac{1}{z} - 2 \frac{\ebz}{z^2} \right] \cdot dz
	\end{align} 

\newcard 

\begin{align}
	\frac{dy}{dx} &= -\frac{2\left(\yx \right)\cdot e^\xy}{\left( \yx - 2\cdot e^\xy\right) } \\
	\text{and if } z &= \yx \text{ then } \\
	\frac{dy}{dx} &= \underbrace{z + x\frac{dz}{dx}}_{ y = z\cdot x} = - \frac{2z\cdot \ebz}{z - 2\cdot \ebz} \\
	x \frac{dz}{dx} &= \frac{-2z\cdot \ebz -z^2 + 2z\cdot\ebz}{z-2\cdot \ebz} \\
	&= -\frac{z^2}{z-2\cdot\ebz} \\
	\therefore -\frac{dx}{x} &= \left[\frac{z-2\cdot \ebz}{z^2} \right]\cdot dz \\
	&= \left[\frac{1}{z} - \frac{2\ebz}{z^2} \right]\cdot dz
\end{align}

\newcard 

\begin{align}
\log y &= 2 \int \frac{\ebz}{z^2}\cdot dz  
\end{align}

\newcard 

\begin{align}
\log y &= -2\int \frac{\ebz}{z^2}\cdot dz 
\end{align}

\newcard 

\begin{align}
-\frac{dx}{x} &= \left[\frac{1}{z} - \frac{2\ebz}{z^2} \right]\cdot dz \\
\therefore \frac{dx}{x} + \frac{dz}{z} &= \frac{2\ebz}{z^2}\cdot dz \\
\therefore \int \frac{dx}{x} + \int \frac{dz}{z} &= \int \frac{2\ebz}{z^2}\cdot dz \\
\text{or } \log x + \log z &= \int \frac{2\ebz}{z^2}\cdot dz  \\
\implies \log \left(x\cdot z \right) &= \log y = \int \frac{2\ebz}{z^2}\cdot dz 
\end{align}

\newcard 

\begin{align}
\int \frac{2\ebz}{z^2}\cdot dz &= -2\cdot e^\xy + C \\
\therefore \log y &= -2e^\xy + C 
\end{align}

\newcard 

\begin{align}
\frac{d}{dx}\frac{1}{z} &= -\frac{1}{z^2} \\
\therefore\text{ if }w &= \frac{1}{z}\text{ then } \frac{dz}{z^2} = -dw \\
\text{and } \int \frac{2\ebz}{z^2}\cdot dz &= -2\int e^w\cdot dw \\
&= -2 e^w + C = -2\ebz + C\\
&= \underbrace{-2\cdot e^\xy + C }_{z = \frac{y}{x}} \\
\text{Hence } \log y &= -2\cdot e^\xy + C 
\end{align}

\newcard 

Given that $x=0$ when $y=1$ 
\[\qquad \log y = 2\cdot \left(1 - e^\xy\right)\]

\newcard 
Given that $x=0$ when $y=1$ 
\[\qquad \log y = 2\cdot \left(\frac{1}{2} - e^\xy\right)\]

\newcard 

We have to find the particular solution. Which means, we need a value for $C$

\begin{align}
x =0\text{ when } &y = 1 \implies \log 1 = -2\cdot e^{\frac{0}{1}} + C \\
\therefore C &= 0 + 2 = 2 \quad (\because \log 1 = 0) \\
\text{Hence } \log y &= -2\cdot e^\xy + 2 = 2\cdot \left(1-e^\xy \right)
\end{align}
\end{document}