\documentclass[14pt,fleqn]{extarticle}
\RequirePackage{prepwell}
\previewoff
\begin{document}

Evaluate the following integral 
\[ \quad R = \int_0^{\frac\pi{2}} \left(2\log\sin x - \log\sin 2x \right)\cdot dx \] 

\newcard 
\begin{align}
	2\log \left( \sin x \right) - \log \left(\sin 2x \right) &= \log \left(\tan x \right) - \log 2 
\end{align}

\newcard 

\begin{align}
	2\log \left( \sin x \right) - \log \left(\sin 2x \right) &= 
	2\log \left(\sin x \right) \\
	&-\left[\log 2 + \log \sin x \right] \\ 
	&= \log \left(\sin x \right) -\log 2 
\end{align}

\newcard 

Just simple algebra involving $\log$ terms
\begin{align}
	2\log \left( \sin x \right) &- \log \left(\sin 2x \right) =\log \left(\sin^2 x \right)-\log \left(\sin 2x \right) \\
	&= \log \left[\dfrac{\sin^2 x}{\sin 2x} \right] = \log \left[\dfrac{\sin^2 x}{2\sin x \cdot\cos x}\right] \\
	&= \log \left[\dfrac{\tan x}{2} \right] = \log \left(\tan x \right)-\log 2
\end{align}

\newcard 

\begin{align}
R &= \int_0^{\frac\pi{2}} \left[\log \left(\tan x \right) - \log 2 \right]\cdot dx \\
&= \underbrace{\int_0^{\frac\pi{2}}\log \left(\tan x \right)\cdot dx}_{A} - \int_0^{\frac\pi{2}}\log 2\cdot dx \\
\text{And } A &= \int_0^{\frac\pi{2}}\log \left(\tan x \right)\cdot dx 
=\int_0^{\frac\pi{2}}\log \left(\cot x \right)\cdot dx \\
\therefore A &= 0 \implies R = -\frac\pi{2}\cdot\log 2
\end{align}

\newcard 

This step is about using the standard result 
\[\qquad \int_0^a f(x)\cdot dx = \int_0^a f \left(a-x \right)\cdot dx  \]

So, starting with $R$ 
\begin{align}
R &= \int_0^{\frac\pi{2}} \left[\log \left(\tan x \right) - \log 2 \right]\cdot dx \\
&= \underbrace{\int_0^{\frac\pi{2}}\log \left(\tan x \right)\cdot dx}_{A} - \int_0^{\frac\pi{2}}\log 2\cdot dx \\
\text{But } A &= \int_0^{\frac\pi{2}}\log \left(\tan x \right)\cdot dx 
\\
&=\int_0^{\frac\pi{2}}\log \left[\tan \left(\frac\pi{2} - x \right)\right] \cdot dx \\
&= \int_0^{\frac\pi{2}}\log \left(\cot x \right)\cdot dx  \\
\therefore A + A  &= \int_0^{\frac\pi{2}} \left[\log \left(\tan x \right) + \log \left(\cot x \right) \right]\cdot dx \\
&= \int_0^{\frac\pi{2}} \log \left(\tan x\cdot \cot x \right)\cdot dx \\ 
&= \int_0^{\frac\pi{2}} \log 1\cdot dx = 0 \quad (\because \log 1 = 0) \\
\text{Hence } R &= A - \log 2\int_0^{\frac\pi{2}} dx = 0 - \log 2\cdot \frac\pi{2} \\
&= -\frac\pi{2}\cdot \log 2 
\end{align}
\end{document}