\documentclass[14pt,fleqn]{extarticle}
\RequirePackage{prepwell}
\previewoff

\newcommand\xmtw{ \left(x-2 \right)}
\newcommand\xptw{ \left(x + 2 \right)}
\newcommand\xmth{ \left(x-3 \right)}
\newcommand\xpth{\left(x+3 \right) }
\newcommand\xsqtw{ \left(x^2 - 4 \right) }
\newcommand\xsqth{ \left(x^2 - 9 \right)}

\begin{document}

\begin{question}
	\statement 
    
    Solve the following equation 
    \[ \tan^{-1} \left(\frac{x-2}{x-3} \right) + \tan^{-1} \left(\frac{x+2}{x+3} \right) = \frac\pi{4} \]
    given that $x \geq 0$ 
    
    \begin{step}
  \begin{options} 
     \correct 
       \small\[ \tan^{-1} \left(\frac{x-2}{x-3} \right) + \tan^{-1} \left(\frac{x+2}{x+3} \right) = \tan^{-1} \left( \frac{2x^2 - 12}{-5}\right)\]
     \incorrect
        
        \[ \tan^{-1} \left(\frac{x-2}{x-3} \right) + \tan^{-1} \left(\frac{x+2}{x+3} \right) = \tan^{-1} \left( \frac{x^2 - 6}{5}\right)\]
    \end{options} 
     \reason 
     
     \begin{align}
	&\tan^{-1} A + \tan^{-1} B = \tan^{-1} \left(\frac{A + B}{1-A\cdot B} \right) \\
	&\therefore \tan^{-1} \left(\frac{x-2}{x-3} \right) + \tan^{-1} \left(\frac{x+2}{x+3} \right) \\
	&= \tan^{-1} \left[ \frac{\frac{x-2}{x-3} + \frac{x+2}{x+3}}{1- \left(\frac{x-2}{x-3} \right)\cdot \left(\frac{x+2}{x+3} \right)} \right]  \\
	&= \tan^{-1} \left[ \frac{\frac{\left(x^2+x-6 \right) + \left(x^2 - x - 6 \right)}{\xsqth}}{\frac{\xsqth-\xsqtw}{\xsqth}} \right] \\
	&= \tan^{-1} \left[\frac{2x^2 - 12}{-5} \right]
\end{align}
       
\end{step}     

\begin{step}
  \begin{options} 
     \correct 
       
       \[ \tan^{-1} \left(\frac{2x^2-12}{-5} \right) = \frac\pi{4} \implies x = \frac{\sqrt{7}}{\sqrt{2}} \]
     \incorrect
        
         \[ \tan^{-1} \left(\frac{2x^2-12}{-5} \right) = \frac\pi{4} \implies x = \frac{\sqrt{3}}{\sqrt{2}} \]
    \end{options} 
     \reason 
       
       \begin{align}
       \tan^{-1} \left(\frac{2x^2-12}{-5} \right) &= \frac\pi{4} \\ 
       \therefore \frac{2x^2 - 12}{-5} &= 1 \\ 
       \implies 2x^2 &= 7\text{ or } x = \pm \frac{\sqrt{7}}{\sqrt{2}}
\end{align}

But as $x \geq 0$, therefore only $x = \frac{\sqrt{7}}{\sqrt{2}}$ is an acceptable solution 
\end{step} 
\end{question} 

\end{document}