

\question[2] Find an expression for the sum of the first $n$ terms of the series 
\[ \dfrac{3}{4} + \dfrac{5}{36} + \ldots + \dfrac{2n+1}{n^2\cdot(n+1)^2} + \ldots \]

\begin{solution}[\halfpage]
  If $a_n$ be the $n-$th term of the series, then 
  \[ a_n = \dfrac{2n+1}{n^2\cdot (n+1)^2} = \dfrac{(n+1)^2-n^2}{n^2\cdot (n+1)^2} = \dfrac{1}{n^2}-\dfrac{1}{(n+1)^2} \] 
  Hence, 
  \begin{align}
    S_n &= \sum_{k=1}^n a_k = \sum_{k=1}^n\left[ \dfrac{1}{n^2} - \dfrac{1}{(n+1)^2} \right] \\
    &= \sum_{k=1}^n \dfrac{1}{n^2} - \sum_{k=1}^n\dfrac{1}{(n+1)^2} \\
    &= \underbrace{\left( 1+\dfrac{1}{2^2}+ \ldots +\dfrac{1}{n^2} \right) - 
       \left( \dfrac{1}{2^2}+\dfrac{1}{3^2} + \ldots +\dfrac{1}{n^2} + \dfrac{1}{(n+1)^2} \right)}
       _{\text{middle terms cancel out}} \\
    &= 1-\dfrac{1}{(n+1)^2} = 
    \dfrac{n\cdot (n+2)}{(n+1)^2}
  \end{align} 
\end{solution}
\ifprintanswers\begin{codex}$\dfrac{n\cdot (n+2)}{(n+1)^2}$\end{codex}\fi
