\documentclass[14pt,fleqn]{extarticle}
\RequirePackage{prepwell}

\previewoff

\begin{document} 

\begin{snippet}
    \incorrect
    
\[ \lim_{x\to\frac\pi{2}}\left(\dfrac{\cos x}{x-\frac\pi{2}}\right) = 1 \]
    
    \reason

\begin{align}
\text{Let }z = x-\frac\pi{2}&\implies x = z + \frac\pi{2} \\ 
\text{Also, as }x\to\frac\pi{2} &, z\to 0  \\
\therefore  \lim_{x\to\frac\pi{2}}\left(\dfrac{\cos x}{x-\frac\pi{2}}\right) &= 
\lim_{z\to 0}\left[\dfrac{\cos\left( z+\frac\pi{2}\right)}{z}\right] \\
&= \underbrace{\lim_{z\to 0}\dfrac{-\sin z}{z}}_{\cos\left(\frac\pi{2}+\theta\right) = -\sin\theta} \\
&= -1\cdot\lim_{z\to 0}\dfrac{\sin z}{z} = -1 
\end{align}   
 
\end{snippet} 
\end{document} 