\documentclass[14pt,fleqn]{extarticle}
\RequirePackage{prepwell-eng}

\previewoff 

\begin{document} 
\begin{snippet}
    \correct
    
    If $\prob{A} = \dfrac{1}{2}, \prob{B} = \dfrac{1}{3}$ and $\prob{A\cap B}=\dfrac{1}{4}$, then $\condp{A'}{B} = \dfrac{1}{4}$ 
    
    \reason
    
    From Bayes' Theorem, we know that 
    \[\qquad \condp{A'}{B} = \dfrac{\prob{A'\cap B}}{\prob{B}} \]
    
    So, to find $\condp{A'}{B}$, we need to first know that $\prob{A'\cap B}$ is \newline 
    
    Hence, the figure below. Notice that 
    \[\qquad A'\cap B = B - \left(A\cap B \right)\]
    \begin{center}
\includegraphics[scale=2]{100-A.eps}
\end{center}

And therefore 
\begin{align}
	\condp{A'}{B} &= \dfrac{\prob{A'\cap B}}{\prob{B}} \\
	&= \dfrac{\prob{B} - \prob{A\cap B}}{\prob{B}} \\
	&= 1- \dfrac{\prob{A\cap B}}{\prob{B}} = 1- \dfrac{\frac{1}{4}}{\frac{1}{3}} \\
	&= 1-\frac{3}{4} = \frac{1}{4} 
\end{align}
    
\end{snippet} 
\end{document} 
