\documentclass[14pt,fleqn]{extarticle}
\RequirePackage{prepwell}

\previewoff

\begin{document} 

\begin{snippet}
    \correct

Given that $ e^x = 1 + x + \frac{x^2}{2!} + \frac{x^3}{3!} + \ldots$
\[\qquad \qquad \lim_{x\to 0}\dfrac{e^x-1}{x} = 1 \]
        
    \reason


\begin{align}
e^x - 1 &= \left( 1 + x + \frac{x^2}{2!} + \frac{x^3}{3!} + \ldots\right) - 1 \\ 
&= x + \frac{x^2}{2!} + \frac{x^3}{3!} + \ldots \\
&= x\cdot\left( 1 + \frac{x}{2!} + \frac{x^2}{3!} + \ldots\right) \\
\therefore \lim_{x\to 0}\dfrac{e^x-1}{x} &= \lim_{x\to 0}\left( 1 + \frac{x}{2!} + \frac{x^2}{3!} + \ldots\right) = 1
\end{align}
    
\end{snippet} 
\end{document} 