\documentclass[14pt,fleqn]{extarticle}
\RequirePackage{prepwell-eng}

\newcommand\pt{\left(1,\frac\pi{4} \right)}
\newcommand\yx{\frac{y}{x}}
\newcommand\dvdx{\frac{dv}{dx}}

\previewoff

\begin{document} 
\begin{problem}
	\statement 
    
    Find the equation of the curve passing through $\pt$ if the slope of the
    tangent of the curve at any point $P(x,y)$ is $\yx -\cos^2\yx$ 
    
    \begin{step}
  \begin{options} 
     \correct 
       
       We have been told that 
       \[ \qquad \dydx = \yx - \cos^2 \yx \]
     \incorrect
        
       We have been told that 
       \[ \qquad P(x,y) = \yx - \cos^2\yx \] 
    \end{options} 
     \reason 
     
     It is some curve in the $x-y$ plane. We don't know what it looks like. But we have been told the \underline{slope of the tangent} at any point\newline 
     
     In other words, we have been told what $\dydx$ is. And it is, 
     
     \[ \qquad\qquad  \dydx = \yx - \cos^2\yx \]
       
\end{step}

\begin{step}
  \begin{options} 
     \correct 
      
      \[ \qquad \underbrace{\dydx = \yx - \cos^2\yx}_{\text{Homogenous differential equation}}\]
      
      And hence, if $ y = vx$, then 
      \[ \qquad \sec^2 v \cdot dv = -\frac{dx}{x} \]
     \incorrect
     
      \[ \qquad \underbrace{\dydx = \yx - \cos^2\yx}_{\text{Homogenous differential equation}}\]
      
      And hence, if $ y = vx$, then 
      \[ \qquad \tan^2 v \cdot dv = -\frac{dx}{x} \]
        
    \end{options} 
     \reason 
     
     \[ \qquad \dydx = \yx - \cos^2\yx = F \left(\yx \right)\]
     Hence, this is obviously a \underline{homogenous} differential equation \newline 
     
     And to solve such a differential equation, we let $y = vx$. Hence, 
     \begin{align}
     y = vx &\implies \underbrace{\dydx = v + x\dvdx}_{\text{Product Rule}} \\
     \therefore v + x\dvdx &= \yx - \cos^2\yx = v - \cos^2 v \\
     \frac{dv}{\cos^2 v} &= -\frac{dx}{x} \text{ or } \sec^2 v\cdot dv = -\frac{dx}{x}
\end{align}
       
\end{step}

\begin{step}
  \begin{options} 
     \correct 
      
      \[ \qquad \sec^2v \cdot dv = -\frac{dx}{x}\quad \left(v = \yx \right) \] 
      And as the curve passes through $\pt$, therefore the required curve is 
      \[ \qquad \tan\yx + \log x = 1 \]
       
     \incorrect
     
     \[ \qquad \sec^2v \cdot dv = -\frac{dx}{x}\quad \left(v = \yx \right) \] 
      And as the curve passes through $\pt$, therefore the required curve is 
      \[ \qquad \tan\yx = -\log x \]
        
    \end{options} 
     \reason 
     
     \begin{align}
	\sec^2 v\cdot dv &= -\frac{dx}{x} \\
	\implies \int \sec^2v\cdot dv &= -\int \frac{dx}{x}\\
	\text{or } \tan v &= -\log x + C \\
	\text{or }\tan\yx + \log x &= C \quad \left(\because v = \yx \right) \\
\end{align}\\[-40pt]
    
    But as the curve passes through $\pt$, therefore
    \begin{align}
    \tan \left(\dfrac{\frac\pi{4}}{1} \right) + \log 1 &= C \\
    \implies C &= \tan\frac\pi{4} = 1 
\end{align}

    And hence, the required curve is 
    \[ \qquad \tan\yx + \log x = 1 \]
       
\end{step}

          
\end{problem} 
\end{document} 