\documentclass[14pt,fleqn]{extarticle}
\RequirePackage{prepwell}
\previewoff
\begin{document}
\begin{question}
\statement
	
%text
Solve the following differential equation 
\[ \qquad (x^2-y^2)\cdot dx +2xy\cdot dy = 0 \]
given that $y=1$ when $x=1$
%
\begin{step}
	\begin{options}
		\correct

		\[\dydx = F\left( \frac{y}{x}\right) = \dfrac{\left(\frac{y}{x}\right)^2 - 1}{2\frac{y}{x}} \]
		And hence, this is a \underline{homogenous} differential equation

		\incorrect
		
		\begin{align}
		\left(x^2-y^2 \right) dx + 2xy\cdot dy &= 0  \\
		\implies 2xy\cdot\dydx - y^2 &= -x^2 
\end{align}

And hence, this is a \underline{first-order linear} differential equation

	\end{options}
	\reason

	%text
Just a little algebra is required here. 

%
\begin{align}
(x^2-y^2)\cdot dx &+2xy\cdot dy = 0 \\
\therefore 2xy\frac{dy}{dx} &= (y^2-x^2)  \\ 
\implies \frac{dy}{dx} &= \underbrace{\dfrac{\left[\left( \frac{y}{x}\right)^2 - 1\right]\cdot x^2}{2\frac{y}{x}\cdot x^2}}_{\text{Factor out $x^2$}}\\
\implies \frac{dy}{dx} &= 
\underbrace{\dfrac{\left(\frac{y}{x}\right)^2 - 1}{2\frac{y}{x}}}_{F\left( \frac{y}{x}\right)}
\end{align}

The fact that $\dydx = F \left(\frac{y}{x} \right)$ makes this a 
\underline{homogenous} differential equation

\end{step}
\begin{step}
	\begin{options}
		\correct

		\[\text{If } y = vx\text{ then } \frac{2v}{1+v^2}\cdot dv = -\frac{dx}{x}\]

		\incorrect

		\[\text{If } y = vx\text{ then }\frac{2v}{1- v^2}\cdot dv = \frac{dx}{x}\]

	\end{options}
	\reason

	\begin{align}
y = vx &\implies \frac{dy}{dx} = v + x\cdot\frac{dv}{dx} \\[5pt]
\therefore  \underbrace{v + x\cdot\frac{dv}{dx}}_{\frac{dy}{dx}} &= F\left(\frac{y}{x}\right) = \frac{v^2-1}{2v} \\
\implies x\cdot\frac{dv}{dx} &= \frac{v^2-1}{2v}- v = -\frac{1+v^2}{2v} \\
\therefore \frac{2v}{1+v^2}\cdot dv &= -\frac{dx}{x} 
\end{align} 
\end{step}
\begin{step}
	\begin{options}
		\correct
		
		\begin{align}
	\frac{2v}{1+v^2} \cdot dv &= -\frac{dx}{x} \\ 
	\implies \int \frac{2v}{1+v^2} \cdot dv &= -\int \frac{dx}{x} \\[5pt]
	\therefore \left(1+v^2 \right)\cdot x &= C \text{ (a constant) }
\end{align}

	\end{options}
	\reason

	\begin{align}
\frac{2v}{1+v^2}\cdot dv &= -\frac{dx}{x} \\
\text{Let } z &= 1+v^2\\
\implies dz &= 2v\cdot dv \\[5pt]
\therefore \frac{dz}{z} &= -\frac{dx}{x}\\
\implies \int\frac{dz}{z} &= -\int\frac{dx}{x} \\
\text{or } \log \vert z\vert &= -\log\vert x\vert + C_1 \\
\implies \log\vert z\vert + \log\vert x\vert &= \log\vert z\cdot x\vert = C_1 \\
\text{or } \underbrace{(1+v^2)}_{ = z}\cdot x &= \underbrace{e^{C_1} = C}_{\log b = a\implies b = e^a}
\end{align} 
\end{step}
\begin{step}
	\begin{options}
		\correct
		
		And therefore, the \underline{specific} solution of the given differential equation is  
		\[\qquad\qquad x^2 + y^2 = 2x \]

	\end{options}
	\reason

	%text
\underline{Do not forget that $y=1$ when $x=1$}

\begin{align}
(1+v^2)\cdot x &= C \\
\implies \left( 1 + \frac{y^2}{x^2}\right)\cdot x &= C\\
\text{And if }y = 1& \text{ when }x = 1 \text{ then}  \\
\left( 1 + \frac{1^2}{1^2}\right)\cdot 1 &= C \implies C = 2 \\
\therefore \left( 1 + \frac{y^2}{x^2}\right)\cdot x &= 2 \\[10pt]
\text{or }x^2 + y^2 &= 2x 
\end{align} 
\end{step}
\end{question}
\end{document}
