

\question[3] If $x^{2x}-2x^{x}\cot y - 1 = 0$, then what is $y'(1)$?
\texttt{Hint:}$\dfrac{d}{dx}x^{Nx}\neq Nx\times x^{Nx-1}$


\ifprintanswers
  % stuff to be shown only in the answer key - like explanatory margin figures
\fi 

\begin{solution}[\halfpage]
  The hint suggests that we need to think about $\dfrac{dz}{dx}$ when $z=x^{Nx}$. So, lets work that out first 
  \begin{align}
    z = x^{Nx} &\implies \ln z = Nx\times\ln x \\
    \implies \dfrac{dz}{dx} &= N\cdot\left[ x\cdot\dfrac{d}{dx}\ln x + \ln x\cdot\dfrac{d}{dx}x\right] \\
    \implies \dfrac{dz}{dx} &= Nx^{Nx}\cdot(1+\ln x)
  \end{align}
  
  Now, coming back to the original equation
	\begin{align}
	  x^{2x}-2x^{x}\cot y - 1 &= 0 \implies
	  \cot y = \dfrac{1}{2}\left[x^{x}-\dfrac{1}{x^{x}} \right] \\
	  &= \dfrac{1}{2}\cdot(x^x-x^{-x}) \\
	  \implies\cot y &= 0 \text{ when } x = 1
	\end{align}
	
	Bearing (3) in mind, we get 
	\begin{align}
	  \dfrac{d}{dx}\cot y &= \dfrac{1}{2}\dfrac{d}{dx}(x^x-x^{-x}) \\
	  \implies -\csc^2 y\dfrac{dy}{dx} &= -(1+\cot^2 y)\dfrac{dy}{dx} \nonumber\\ 
	  &= \dfrac{1}{2}\left[ \underbrace{(1+\ln x)\cdot x^x}_{\frac{d}{dx}x^x} + 
	  \underbrace{(1+\ln x)\cdot x^{-x}}_{\frac{d}{dx}x^{-x}}\right] \\
	  &= \dfrac{(1+\ln x)}{2}\cdot\left(x^x + \dfrac{1}{x^x}\right)
	\end{align}
	
	And therefore, when $x=1$, then 
	\begin{align}
	  \underbrace{-(1+\cot^2 y)}_{\cot y = 0\text{ when } x=1}\dfrac{dy}{dx} &= 
	  \dfrac{1+0}{2}\cdot (1+1) \\
	  \implies \dfrac{dy}{dx} &= -1 \text{ when } x=1
	\end{align}	
\end{solution}
