

\question[4] Evaluate the following limit using L'Hospital's Rule
\[\limit{x}{\infty}\left( 1-\frac{1}{x}\right)^x\] 
\textbf{Hint:} If $\ln f(x)=X$, then $f(x) = e^X = e^{\ln f(x)}$

\begin{solution}[\halfpage]
  Given that,  
  \begin{align}
    f(x) &= e^{\ln f(x)} \\
    \limit{x}{\infty} f(x) &= \limit{x}{\infty} e^{\ln f(x)} = e^{\limit{x}{\infty}\ln f(x)}
  \end{align} 

  we can re-write the original expression as 
  \begin{align}
    \limit{x}{\infty}\left( 1-\frac{1}{x} \right)^x &= e^{\limit{x}{\infty}\ln\left( 1-\frac{1}{x} \right)^x}
  \end{align}

  which gives us 
  \begin{align}
    \limit{x}{\infty}\ln\left( 1-\frac{1}{x} \right)^x &= \limit{x}{\infty}x\cdot\ln\left( 1-\frac{1}{x}\right) \\
    &= \limit{x}{\infty}\dfrac{\ln\left(1-\frac{1}{x}\right)}{\frac{1}{x}}
  \end{align}

  Applying L'Hospital's Rule to the last equation, we get 
  \begin{align}
    \limit{x}{\infty}\dfrac{\ln\left(1-\frac{1}{x}\right)}{\frac{1}{x}} 
    &= \limit{x}{\infty}\dfrac{\frac{1}{\left( 1-\frac{1}{x}\right)}\cdot\frac{1}{x^2}}{-\frac{1}{x^2}} \\
    &= \limit{x}{\infty}-\dfrac{1}{\left( 1-\frac{1}{x}\right)} = -1 \\
    \implies 
    \limit{x}{\infty}\left( 1-\frac{1}{x} \right)^x 
    &= e^{\limit{x}{\infty}\ln\left( 1-\frac{1}{x} \right)^x} = e^{-1} = \dfrac{1}{e}
  \end{align}
\end{solution}

\ifprintanswers\begin{codex}$\dfrac{1}{e}$\end{codex}\fi
