

\question[4] Find the value of $M$ in the following equation:
\[\dfrac{\sin(\pi - \alpha)}{\sin\alpha - 
  \cos\alpha\tan\dfrac{\alpha}{2}} + \cos(\pi - \alpha) = M \nonumber\]


\begin{solution}[\halfpage]
  Substitute the values for $\sin(\pi - \alpha)$ and $\cos(\pi - \alpha)$ 
  in the Left Hand Side(L.H.S) of the equation,
  \begin{align}
    \text{L.H.S} &= \dfrac{\sin\alpha}{\sin\alpha -
    				  \cos\alpha\tan\dfrac{\alpha}{2}}
					  - \cos\alpha \\
    &\textit{(substitute $\dfrac{\alpha}{2}$ with $\theta$)} \nonumber \\
				 &= \dfrac{\sin 2\theta}{\sin 2\theta - 
				 	  \cos 2\theta\tan\theta} + \cos 2\theta \\	
				 &= \dfrac{2\sin\theta\cos\theta}{2\sin\theta\cos\theta - 
				 	  \cos 2\theta\dfrac{\sin\theta}{\cos\theta}} 
				 	  - \cos 2\theta \\
				 &= \dfrac{2\cos ^2\theta}{2\cos^2\theta - 
				 	  \cos 2\theta} - \cos 2\theta \\
				 &= \dfrac{2\cos ^2\theta}{2\cos^2\theta - 
				 	  \cos^2\theta + \sin^2\theta} - \cos^2\theta + \sin^2\theta \\
				 &= \dfrac{2\cos^2\theta}{\cos^2\theta + \sin^2\theta} -
				 	  \cos^2\theta + \sin^2\theta \\
				 &= \cos^2\theta + \sin^2\theta = 1
  \end{align}
\end{solution}
\ifprintanswers\begin{codex}$M=1$\end{codex}\fi
