\documentclass[14pt,fleqn]{extarticle}
\RequirePackage{prepwell}
\previewoff 

\begin{document} 
\begin{question}
	\statement 
    
    Given two events $A$ and $B$ such that 
    \[ \prob{A} = \frac{1}{2}, \prob{B} = \frac{1}{3} \text{ and } \prob{A\cap B} = \frac{1}{4} \]
    find the value of $\condp{A'}{B'}$ 
          
          
   \begin{step}
  \begin{options} 
     \correct 
       
       \[ \condp{A'}{B'} = \dfrac{\prob{A'\cap B'}}{1-\prob{B}} \]
       
     \incorrect
        
     \[ \condp{A'}{B'} = \dfrac{\prob{A'\cap B'}}{\prob{B}} \]
     
    \end{options} 
     \reason 
     
     Do the simplest thing first. Apply Bayes' Theorem to expand $\condp{A'}{B'}$
     \begin{align}
	\condp{A'}{B'} &= \dfrac{\prob{A'\cap B'}}{\prob{B'}} = \dfrac{\prob{A'\cap B'}}{\underbrace{1-\prob{B}}_{\prob{B'}}} 
\end{align}
       
\end{step}

\begin{step}
  \begin{options} 
     \correct 
       
       The shaded region in the figure below is $A'\cap B'$ 
       
       \begin{center}
\includegraphics[scale=1.5]{1411-A.eps}
\end{center}
       And hence $\prob{A'\cap B'} =  1-\prob{A\cup B}$ 
       
     \incorrect
        
        The shaded region in the figure below is $A'\cap B'$ 
       
       \begin{center}
\includegraphics[scale=1.5]{1411-B.eps}
\end{center}
       And hence $\prob{A'\cap B'} =  1-\prob{A\cap B}$ 
    \end{options} 
     \reason 
       
     $A'\cap B'$ is the set of all events that are \underline{not} in $A$ and \underline{not} in $B$\newline 
     
     And from De-Morgan's Laws we know that 
     
     \begin{align}
	\left(A\cup B \right)' &= A'\cap B'  \\
	\therefore \prob{A'\cap B'} &= P \left(A\cup B \right)' \\
	&= 1 - \prob{A\cup B}
\end{align}
     
\end{step}

\begin{step}
  \begin{options} 
     \correct 
       
     Therefore $\condp{A'}{B'} = \dfrac{5}{8}$ 
        
    \end{options} 
     \reason 
     
     \begin{align}
	\condp{A'}{B'} &= \dfrac{\prob{A'\cap B'}}{\prob{B'}} \\
	&= \dfrac{1-\prob{A\cup B}}{1-\prob{B}} \\
	\prob{A\cup B} &= \prob{A} + \prob{B} - \prob{A\cap B} \\[-10pt]
	&= \frac{1}{2} + \frac{1}{3} - \frac{1}{4} = \frac{7}{12} \\
	\therefore \condp{A'}{B'} &= \left[\dfrac{1-\frac{7}{12}}{1-\frac{1}{3}}  \right]= \left[\dfrac{\frac{5}{12}}{\frac{2}{3}} \right] = \frac{5}{8}
\end{align}
       
\end{step}
\end{question} 
\end{document} 