
\ifnumequal{\value{rolldice}}{0}{
  \renewcommand\va{A}
  \renewcommand\vb{B}
  \renewcommand\vc{C}
}{
  \ifnumequal{\value{rolldice}}{1}{
    \renewcommand\va{F}
    \renewcommand\vb{G}
    \renewcommand\vc{H}
  }{
    \ifnumequal{\value{rolldice}}{2}{
      \renewcommand\va{P}
      \renewcommand\vb{Q}
      \renewcommand\vc{R}
    }{
      \renewcommand\va{X}
      \renewcommand\vb{Y}
      \renewcommand\vc{Z}
    }
  }
}

\question[4] For the following to be true
\[ (\va-\vb)\cap(\vc-\vb) = \va-(\vb\star\vc ')\]
, the $\star$ should be replaced with which of $\cup$, $\cap$ or $-$ (minus)? 

\watchout

\ifprintanswers
  \begin{marginfigure}
    \begin{venndiagram3sets}[labelA=$\va$,labelB=$\vb$,labelC=$\vc$,labelNotABC=$U$]
      \fillACapCNotB
    \end{venndiagram3sets}
  \end{marginfigure}
\fi

\begin{solution}[\halfpage]
  \begin{align}
    (\va-\vb)\cap(\vc-\vb) &= \overbrace{(\va\cap\vb ')\cap(\vc\cap\vb ')}^{J-K=J\cap K'} \\
    &= \va\cap(\vb '\cap \vb')\cap\vc \\
    &= \va\cap(\vc\cap\vb ') = \va\cap\underbrace{[(\vc\cap\vb')']'}_{K = (K')'}
  \end{align}
  Now, if we let $K = (\vc\cap\vb')'$, then the last equation becomes 
  \begin{align}
    &=\va\cap K' = \va - K = \va - (\vc\cap\vb')' \\
    &= \va - \underbrace{(\vc '\cup\vb)}_{\text{De-Morgan's}}
  \end{align}
  Which means, that we need to replace the $\star$ with $\cup$ (union)
\end{solution}

\ifprintanswers\begin{codex}$\cup\text{ (union)}$\end{codex}\fi
