\documentclass[14pt,fleqn]{extarticle}
\RequirePackage{prepwell}
\previewoff
\begin{document}

%text
Write the principal value of $\sec^{-1}(-2)$. 
%
%
\newcard 

\[ \sec^{-1} (-2) = \cos^{-1} \left(-\frac{1}{2} \right)\]

\newcard 

\[ \sec^{-1} (-2) = -\cos^{-1} \left(\frac{1}{2} \right)\]

\newcard 

The standard result is $\sec^{-1} x = \cos^{-1} \left(\frac{1}{x} \right)$ \newline 

In this case $x = -2$\newline 
And therefore $\sec^{-1} (-2) = \cos^{-1} \left(\frac{-1}{2} \right)$ \newline 

\newcard 
\[ \cos \left(\frac{8\pi}{3} \right) = -\frac{1}{2} \implies\cos^{-1} \left( \frac{-1}{2}\right) = \frac{8\pi}{3}\]

\newcard 

When we say that $\cos^{-1}x = \theta$, then $\theta$ belongs to what is called the \underline{principal range}. For $\cos^{-1}x$, that principal range is $[0,\pi]$\newline 

And it so happens that 
\begin{align}
\cos \frac{2\pi}{3} = -\frac{1}{2} &\text{ and } \frac{2\pi}{3}\in [0,\pi] \\
\therefore \cos^{-1} \left(\frac{-1}{2} \right) &= \frac{2\pi}{3}
\end{align}


\end{document}