

\ifnumequal{\value{rolldice}}{0}{
  % variables 
  \renewcommand{\va}{2}
}{
  \ifnumequal{\value{rolldice}}{1}{
    % variables 
    \renewcommand{\va}{4}
  }{
    \ifnumequal{\value{rolldice}}{2}{
      % variables 
      \renewcommand{\va}{3}
    }{
      % variables 
      \renewcommand{\va}{5}
    }
  }
}

\ADD\va{1}\vb
\ADD\va{2}\vc
\ADD\va{3}\vd
\ADD\va{4}\ve

\question[3] Find an expression for the sum of the first $n$ terms of the series 
 \[ \dfrac{1}{\vb\cdot\vc} + \dfrac{1}{\vc\cdot\vd} + \dfrac{1}{\vd\cdot\ve}\ldots \]

\watchout

\begin{solution}[\halfpage]
	 $a_n = \dfrac{1}{(n+\va)\cdot(n+\vb)},\, n \geq 1, n\in\mathbb{N}$ in the above series. 

	 The sum of the first $n$ terms, therefore, is given by 
	 \begin{align}
	 	S_n &= \sum_{k=1}^{n}\dfrac{1}{(k+\va)\cdot(k+\vb)} =
	 	  \sum_{k=1}^{n}\dfrac{k+\vb - (k+\va)}{(k+\va)\cdot(k+\vb)} \\
	 	&= \sum_{k=1}^{n}\dfrac{1}{k+\va} - \sum_{k=1}^{n}\dfrac{1}{k+\vb} \\
	 	&= \underbrace{\left( \frac{1}{\vb} + \frac{1}{\vc} + \frac{1}{\vd} + \ldots + \frac{1}{n+\va}\right) - 
	 	\left( \frac{1}{\vc} + \frac{1}{\vd} + \ldots + \frac{1}{n+\va} + \frac{1}{n+\vb}\right)}_{\text{middle terms cancel out}} \\
	 	&= \dfrac{1}{\vb} - \dfrac{1}{n+\vb} = 
    \dfrac{n}{\vb\cdot(n+\vb)}
	 \end{align}
\end{solution}

\ifprintanswers
  \begin{codex}
    $\dfrac{n}{\vb\cdot(n+\vb)}$
  \end{codex}
\fi
