\documentclass[14pt,fleqn]{extarticle}
\RequirePackage{prepwell-eng}

\previewoff 

\begin{document} 
\begin{snippet}
    
    \incorrect
    
    If $f(x) = \dfrac{1}{x}$, then $\dfrac{d}{dx} \left(f\circ f \right)(x) = -\dfrac{1}{x^2}$ 
    \reason
    
    The first question is, what is $\left(f\circ f \right)(x)$? 
    \begin{align}
	   \left(f\circ f \right)(x) &= f \left(\, f(x) \,\right) \\
	   &= f \left(\frac{1}{x} \right) = \dfrac{1}{\frac{1}{x}} = x 
\end{align}

And so, if $ \left(f\circ f \right)(x) = x$, then 
\[ \quad\qquad \ddx \left(f\circ f \right)(x) = 1 \]
    
\end{snippet} 
\end{document} 