\documentclass[14pt,fleqn]{extarticle}
\RequirePackage{prepwell}

\previewoff 

\begin{document} 
\begin{snippet}
    
    \incorrect
    
    \[ y^2\dydx\ + y^2 + 1 = 0 \implies y -x = \tan^{-1} y + C\]
    \reason
    
    \begin{align}
	y^2 \cdot \dydx + y^2 + 1 &= 0 \\
	\therefore \frac{y^2}{y^2+1}\cdot\dydx + 1 &= 0 \\
	\text{or }\dfrac{y^2}{y^2+1}\cdot dy &= -dx  \\
	\left[1 - \frac{1}{y^2+1} \right] dy &= -dx \\
	\text{Hence }\int dy - \int \frac{dy}{y^2+1} &= -\int dx \\
	\text{or } y - \tan^{-1} y &= -x + C \\
	\implies x + y &= \tan^{-1} y + C 
\end{align}
    
\end{snippet} 
\end{document} 