\documentclass[14pt,fleqn]{extarticle}
\RequirePackage{prepwell}
\previewoff
\begin{document}

\newcommand\ea{ \left(x^2+4 \right)}
\newcommand\eb{ \left(x^2 + 9 \right)}
\newcommand\fa{ \frac{4}{5} }
\newcommand\fb{ \frac{9}{5} }
\newcommand\ec{ \frac{x^2}{\ea\cdot\eb} }

%text
Evaluate the following \[\qquad I = \int \frac{x^2}{\ea\cdot\eb}\cdot dx\]
%

\newcard 

\[ \frac{x^2}{\ea\cdot\eb} = \frac{x+B}{\ea} + \frac{x+D}{\eb}\]

\newcard 

We know that 
\[ \frac{x^2}{\ea\cdot\eb} = \frac{Ax + B}{\ea} + \frac{Cx + D}{\eb}\]

But \underline{just by looking} at the above, we can say that $A=C=0$. How? \newline 

Because if we let $z = x^2$, then 
\begin{align}
	\frac{x^2}{\ea\cdot\eb} &= \frac{z}{\left(z+4 \right)\cdot \left(z+9 \right)}\\
	&= \frac{B}{z+4} + \frac{D}{z+9} \\
	&= \frac{B}{\ea} + \frac{C}{\eb}
\end{align}

We have therefore reduced our work to finding just $B$ and $D$ \newline 

\newcard

\[ \ec = -\frac{\fa}{\ea} + \frac{\fb}{\eb}\]

\newcard 

\[ \ec = \frac{\fa}{\ea} + \frac{\fb}{\eb} \]

\newcard 

\begin{align}
	\ec &= \frac{B}{\ea} + \frac{D}{\eb} \\
	\therefore x^2 &= B\eb + D\ea \\
	&= (B+D)x^2 + (9B+4D)
\end{align}

On \underline{comparing coefficients}, we see that 
\begin{align}
	B + D &= 1 \text{ and } 9B + 4D = 0 \\
	\therefore B &= -\fa\text{ and } D = \fb 
\end{align}

Hence 
\[ \ec = -\frac{\fa}{\ea} + \frac{\fb}{\eb}\]

\newcard 

\begin{align}
	I &= -\fa\int \frac{dx}{\ea} + \fb\int \frac{dx}{\eb} \\
	&= \frac{1}{5} \left[3\tan^{-1}\frac{x}{3} - 2\tan^{-1}\frac{x}{2} \right] + C
\end{align}

\newcard 

\begin{align}
I &= -\fa\int \frac{dx}{\ea} + \fb\int \frac{dx}{\eb} \\
&= \frac{1}{5} \left[-4\int \frac{dx}{\ea} + 9\int \frac{dx}{\eb} \right]\\
&= \frac{1}{5} \underbrace{\left[-4 \left(\frac{1}{2}\tan^{-1}\frac{x}{2} \right) + 9 \left(\frac{1}{3}\tan^{-1}\frac{x}{3} \right)\right]}_{\int \frac{dx}{x^2+a^2} = \frac{1}{a}\tan^{-1}\frac{x}{a} + C} + C\\
	&= \frac{1}{5} \left[3\tan^{-1}\frac{x}{3} - 2\tan^{-1}\frac{x}{2} \right] + C
\end{align}

\end{document}