


\ifnumequal{\value{rolldice}}{0}{
  \renewcommand{\va}{63}
}{
  \ifnumequal{\value{rolldice}}{1}{
    \renewcommand{\va}{64}
  }{
    \ifnumequal{\value{rolldice}}{2}{
      \renewcommand{\va}{65}
    }{
      \renewcommand{\va}{66}
    }
  }
}

\SUBTRACT\va{1}\vb

\question[3] Differentiate $y=\cos^2(x^{\va})$ with respect to $x$.

\watchout

\begin{solution}[\halfpage]
  If $z = \cos(x^{\va})$, then $y = z^2$ and \textbf{chain-rule} tells us that 
  \begin{align}
    \dydx &= \dfrac{\mathrm{d}}{\mathrm{d}z}z^2\cdot\dydx[z] \\
    &= 2z\cdot\dydx[\cos(x^{\va})] \\
    &= \underbrace{(2\cos x^{\va})\cdot(-\sin x^{\va})}_{2\sin\theta\cos\theta = \sin 2\theta}\cdot\va\cdot x^{\vb} \\
    &= -\va\cdot x^{\vb}\cdot\sin (2x^{\va})
  \end{align}
  \textbf{Alternatively,} one could also say that given $\cos^2 x = \dfrac{\cos 2x + 1}{2}$,
  \begin{align}
    \dydx &= \dydx[\left( \dfrac{\cos 2x^{\va} + 1}{2}\right)] 
    = \dfrac{1}{2}\dydx[\cos 2x^{\va}] \\
    &= \dfrac{1}{2}\cdot (-\sin 2x^{\va} )\cdot\dydx[2x^{\va}] \\
    &= \dfrac{1}{2}\cdot (-\sin 2x^{\va} )\cdot (2\cdot\va\cdot x^{\vb}) \\
    &= -\va\cdot x^{\vb}\cdot\sin (2x^{\va})
  \end{align}
\end{solution}

\ifprintanswers\begin{codex}
 $-\va\cdot x^{\vb}\cdot\sin (2x^{\va})$
\end{codex}\fi
