\documentclass[14pt,fleqn]{extarticle}
\RequirePackage{prepwell-eng}

\previewoff

\begin{document} 

\begin{snippet}
    
    \incorrect

\[ \lim_{x\to 1}\dfrac{x^{\frac{1}{3}}-1}{x^{\frac{1}{4}}- 1} = \dfrac{1}{12} \]    
    \reason

\begin{align}
\dfrac{x^{\frac{1}{3}}-1}{x^{\frac{1}{4}}- 1} &= 
\dfrac{\left(\dfrac{x^{\frac{1}{3}}-1}{x-1}\right)}{\left(\dfrac{x^{\frac{1}{4}}- 1}{x-1}\right)} \\
\therefore \lim_{x\to 1}\dfrac{x^{\frac{1}{3}}-1}{x^{\frac{1}{4}}- 1} &= 
\dfrac{\lim_{x\to 1}\left(\dfrac{x^{\frac{1}{3}}-1}{x-1}\right)}{\lim_{x\to 1}\left(\dfrac{x^{\frac{1}{4}}- 1}{x-1}\right)} \\
&= \dfrac{\frac{1}{3}\cdot 1^{\frac{1}{3}-1}}{\frac{1}{4}\cdot 1^{\frac{1}{4}-1}} = \dfrac{4}{3}
\end{align}
    
\end{snippet} 
\end{document} 