\documentclass[14pt,fleqn]{extarticle}
\RequirePackage{prepwell}
\previewoff
\begin{document}

\newcommand\ea{x^2 + 3x-18} 
\newcommand\dnm{\sqrt{\ea}}

\newcommand\trma{\left(x+\frac{3}{2} \right)}
\newcommand\trmk{ \left(\frac{9}{2} \right)}

Evaluate the following integral 
\[ \qquad I = \int \frac{x-3}{\dnm}\cdot dx \]

\newcard 

If $f(x) = \ea$ then 
\[ \qquad I = \int \frac{x-3}{\sqrt{f(x)}}\cdot dx \]

The best thing to do is express $I$ as follows 
\begin{align}
	I &= \int \frac{A\cdot f'(x) + B}{\sqrt{f(x)}}\cdot dx \\
	&= A \int \frac{f'(x)}{\sqrt{f(x)}}\cdot dx + B\int \frac{dx}{\sqrt{f(x)}}
\end{align}

\newcard 

Different integrals require different strategies to solve \newline 

The given integral is of the form 
\[ \quad I = \int \frac{px+q}{\sqrt{ax^2 + bx + c}}\cdot dx \]

Hence, let $f(x) = ax^2+bx+c$ and express the integral as 

\begin{align}
	I &= \int \frac{A\cdot f'(x) + B}{\sqrt{f(x)}}\cdot dx \\
	&= A \int \frac{f'(x)}{\sqrt{f(x)}}\cdot dx + B \int \frac{dx}{\sqrt{f(x)}}
\end{align}

\newcard 

\begin{align}
f'(x) &= 2x + 3 \\
\therefore x-3 &= \frac{1}{2}\cdot \left(2x+3 \right) - \frac{9}{2} \\
I &= \underbrace{\frac{1}{2}\int \frac{2x+3}{\dnm}\cdot dx}_P \\
&- \underbrace{\frac{9}{2}\int \frac{dx}{\dnm}}_Q 
\end{align}

\newcard 

\begin{align}
f'(x) &= 2x + 3 \\
\therefore x-3 &= \frac{1}{2}\cdot \left(2x+3 \right) - \frac{7}{2} \\
I &= \underbrace{\frac{1}{2}\int \frac{2x+3}{\dnm}\cdot dx}_P \\
&- \underbrace{\frac{7}{2}\int \frac{dx}{\dnm}}_Q 
\end{align}

\newcard 

\begin{align}
\text{If }f(x) &= \ea \\
\text{then }f'(x) &= 2x + 3 \\
\text{hence }x-3 &= A\cdot \left(2x+3 \right) + B \\ 
&= 2Ax + \left(3A + B \right) \\
\therefore 2A &= 1\text{ and } 3A + B = -3 \\
\text{or } A &= \frac{1}{2}\text{ and } B = -\frac{9}{2}
\end{align}

Which is why 
\small\[ I = \underbrace{\frac{1}{2}\int \frac{2x+3}{\dnm}\cdot dx}_P - \underbrace{\frac{9}{2}\int \frac{dx}{\dnm}}_Q \]\normalsize

\newcard 

\[ P = \dnm  + C_1 \]

\newcard 

\[ P = \frac{\left(\ea \right)^{\frac{3}{2}}}{3} + C_1 \]

\newcard 

Recall that $P= A\int \frac{f'(x)}{\sqrt{f(x)}}\cdot dx$. That said 

\begin{align}
	P &= \frac{1}{2}\int \frac{2x+3}{\dnm}\cdot dx \\
	\text{If } z &= \ea\text{ then } I = \frac{1}{2}\int \frac{dz}{\sqrt{z}} \\
	&= \underbrace{\frac{1}{2}\cdot \frac{\sqrt{z}}{\frac{1}{2}}}_{\int x^n\cdot dx = \frac{x^{n+1}}{n+1}} = \sqrt{z} + C_1 \\
	&= \sqrt{\ea} + C_1 
\end{align}

\newcard 

\begin{align}
	Q &= \frac{9}{2}\int \frac{dx}{\dnm} \\
	&= \frac{9}{2}\cdot \log \left\vert \trma + \dnm \right\vert + C_2
\end{align}

And hence 

\begin{align}
I &= P - Q = \dnm \\
&- \log\left\vert\trma + \dnm\right\vert + C 
\end{align}

\newcard 

\begin{align}
	Q &= \frac{9}{2}\int \frac{dx}{\dnm} \\
	&= \frac{9}{2} \int \frac{dx}{\underbrace{\sqrt{\trma^2 - \trmk^2}}_{\text{Complete the squares}}}\cdot dx \\
	&= \frac{9}{2}\cdot \underbrace{\log \left\vert \trma + \dnm \right\vert}_{\int \frac{dx}{\sqrt{x^2-a^2}} = \log\vert x + \sqrt{x^2-a^2}\vert +C } + C_2
\end{align}

And hence 

\begin{align}
I &= P - Q =  \dnm \\
&- \log\left\vert\trma + \dnm\right\vert + C 
\end{align}

\end{document}