

\question[1] Prove the following identity
  \[\dfrac{\sec\theta - \tan\theta}{\sec\theta + \tan\theta} = 1-2\sec\theta\tan\theta + 2\tan^2\theta\]


\ifprintanswers
\fi 

\begin{solution}[\halfpage]
	\begin{align}
	   \dfrac{\sec\theta - \tan\theta}{\sec\theta + \tan\theta} &= 
	   \dfrac{(\sec\theta - \tan\theta)\cdot(\sec\theta - \tan\theta)}
	         {(\sec\theta + \tan\theta)\cdot(\sec\theta - \tan\theta)} \\
	     &= \dfrac{(\sec\theta-\tan\theta)^2}{\underbrace{\sec^2\theta-\tan^2\theta}_{=1}} \\
	     &= \sec^2\theta - 2\sec\theta\tan\theta + \tan^2\theta \\
	     &= (1 + \tan^2\theta) - 2\sec\theta\tan\theta + \tan^2\theta \\
	     &= 1 - 2\sec\theta\tan\theta + 2\tan^2\theta
	\end{align}
\end{solution}
