

\question[3] If $\csc\theta - \sin\theta = a$ and $\sec\theta - \cos\theta = b$, then 
find the value of 
  \[ a^{\frac{2}{3}}\cdot b^{\frac{2}{3}}\cdot(a^{\frac{2}{3}}+b^{\frac{2}{3}}) \]
  \[ (\csc\theta = \text{cosec }\theta) \]

\ifprintanswers
\fi 

\begin{solution}[\halfpage]
	\begin{align}
		\csc\theta - \sin\theta &= \dfrac{1}{\sin\theta} - \sin\theta = a \\
		\implies \dfrac{\cos^2\theta}{\sin\theta} &= a \\
		\text{Similarly, }\sec\theta - \cos\theta &= \dfrac{1}{\cos\theta} - \cos\theta = b \\
		\implies \dfrac{\sin^2\theta}{\cos\theta} &= b \\
		\therefore (a\cdot b)^{\frac{2}{3}}\cdot(a^{\frac{2}{3}} + b^{\frac{2}{3}}) &= 
		\cos^{\frac{2}{3}}\theta\cdot\sin^{\frac{2}{3}}\theta\times
		\left[ \dfrac{\cos^{\frac{4}{3}}\theta}{\sin^{\frac{2}{3}}\theta} + 
		\dfrac{\sin^{\frac{4}{3}}\theta}{\cos^{\frac{2}{3}}\theta}\right] \\
    &= \dfrac{(\cos\theta\cdot\sin\theta)^
    {\frac{2}{3}}\cdot(\cos^{\frac{4}{3}+\frac{2}{3}}\theta + 
    \sin^{\frac{4}{3}+\frac{2}{3}}\theta)}{(\cos\theta\cdot\sin\theta)^{\frac{2}{3}}} \\
		&= \cos^2\theta + \sin^2\theta = 1
	\end{align}
\end{solution}
