
\ifnumequal{\value{rolldice}}{0}{
  \renewcommand\va{6}
}{
  \ifnumequal{\value{rolldice}}{1}{
    \renewcommand\va{4}
  }{
    \ifnumequal{\value{rolldice}}{2}{
      \renewcommand\va{8}
    }{
      \renewcommand\va{10}
    }
  }
}

\DIVIDE\va{2}\vb

\question[2] Evaluate the following 
  \[ \int \va x\tan^{-1}x\ud x \]

\watchout

\begin{solution}[\halfpage]
  If $f(x)$ and $g(x)$ be two functions, then 
  \begin{align}
    \dfrac{d}{dx}f(x)\cdot g(x) &= f'(x)\cdot g(x) + f(x)\cdot g'(x) \\
    \implies f(x)\cdot g(x) &= \int f'(x)\cdot g(x) dx + \int f(x)\cdot g'(x) dx
  \end{align} 

  Now, if we let 
  \begin{align}
    f(x) &= \dfrac{x^2}{2}\implies f'(x) = \dfrac{2x}{2} = x \\
    \text{and } g(x) &= \tan^{-1} x
  \end{align}

  then it would also be true that 
  \begin{align}
    \dfrac{\va x^2}{2}\cdot\tan^{-1}x &= \overbrace{\int \va x\cdot\tan^{-1} x dx}^{\text{what we need}} 
          + \int\dfrac{\va x^2}{2}\cdot\dfrac{d}{dx}\tan^{-1}x dx \\
    \implies \int \va x\cdot\tan^{-1}x dx &= \vb x^2\cdot\tan^{-1}x - \vb\int\dfrac{x^2}{1+x^2} dx \\
        &= \vb x^2\cdot\tan^{-1}x 
          -\vb\int\dfrac{x^2+1-1}{x^2 + 1} dx \\
        &= \vb x^2\cdot\tan^{-1}x 
        - \vb\left[ \int dx - \int\dfrac{1}{1+x^2} dx \right] \\
        &= \vb x^2\cdot\tan^{-1} x -\vb\cdot(x-\tan^{-1}x) + C \\
        &= \vb\left[ (x^2+1)\tan^{-1}x -x \right] + C 
  \end{align}
\end{solution}

\ifprintanswers
  \begin{codex}
    $\vb\left[ (x^2+1)\tan^{-1}x -x \right] + C$
  \end{codex}
\fi
