\documentclass[14pt,fleqn]{extarticle}
\RequirePackage{prepwell-eng}

\newcommand\trma{\frac{e^{-2\sqrt{x}}}{\sqrt{x}}}
\newcommand\trmb{\frac{y}{\sqrt{x}}}

\previewoff 

\begin{document} 
\begin{snippet}
    \correct
    
    The integrating factor $(I)$ of the following differential equation 
    \[ \qquad \left(\trma -\trmb \right)\cdot \frac{dx}{dy} = 1\, (x\neq 0)\]
    is $I = e^{2\sqrt{x}}$ 
    
    \reason
    
    \begin{align}
	\left(\trma - \trmb \right)\cdot \frac{dx}{dy} &= 1 \\
	\implies \trma - \trmb &= \dydx \\
	\text{or } \dydx + \underbrace{\trmb}_{P(x)} &= \trma 
\end{align}
    
This looks like a \underline{first-order} linear differential equation with $P(x) = \frac{1}{\sqrt{x}}$ \newline 

Hence $I = e^{\int P(x)\cdot dx} = e^{\int \frac{dx}{\sqrt{x}}} = e^{2\sqrt{x}}$ 

\end{snippet} 
\end{document} 