\documentclass[14pt,fleqn]{extarticle}
\RequirePackage{prepwell}
\previewoff
\begin{document}

%text
Solve the differential equation
\[ \qquad \frac{dy}{dx} + y = \cos x - \sin x \]
%

\newcard

$\dfrac{dy}{dx} + y = \cos x - \sin x$ is a \underline{linear} differential equation 

\newcard 

$\dfrac{dy}{dx} + y = \cos x - \sin x$ is a \underline{homogenous} differential equation

\newcard 

$\dfrac{dy}{dx} + y = \cos x - \sin x$ looks exactly like
\[ \qquad\qquad \frac{dy}{dx} + y\cdot P(x) = Q(x) \]

which, as you may recall, is a \underline{linear} differential equation \newline 

And therefore, so is $\frac{dy}{dx} + y = \cos x-\sin x$ 

\newcard 

\begin{align}
	\dfrac{dy}{dx} + y &= \cos x - \sin x \\
	\implies \frac{d}{dx} \left(e^x\cdot y \right) &= e^x\cdot \left(\cos x - \sin x \right)
\end{align}

\newcard 

The \underline{integrating factor} $I(x) = e^{\int P(x)\cdot dx}$ , where $P(x) = 1$ (compare with the form of a linear differential equation) \newline 

And hence, $I(x) = e^{\int dx} = e^x$. Which means that when we multiply both sides by $I(x)$, then 

\begin{align}
e^x\cdot \left[\frac{dy}{dx} + y \right] &= e^x\cdot \left(\cos x - \sin x \right) \\
e^x\cdot\frac{dy}{dx} + e^x\cdot y &= e^x\cdot \left(\cos x - \sin x \right) \\
\text{or } \frac{d}{dx} \left(e^x\cdot y \right) &= e^x\cdot \left(\cos x - \sin x \right)
\end{align}

\newcard 
\[ \int e^x\cdot \left(\cos x - \sin x \right)\cdot dx = e^x\cdot \cos x + C \]

And therefore, 
\[ \qquad \qquad y = \cos x + \dfrac{C}{e^x} \]

\newcard 
\[ \int e^x\cdot \left(\cos x - \sin x \right)\cdot dx = -e^x\cdot \sin x + C \]

And therefore, 
\[ \qquad \qquad y = -\sin x + \dfrac{C}{e^x} \]

\newcard 

\begin{align}
\dfrac{d}{dx} \left(e^x\cdot y \right) &= e^x\cdot \left(\cos x - \sin x \right) \\
\implies e^x\cdot y &= \int e^x\cdot \left(\cos x -\sin x \right)\cdot dx \\
\text{And so, } y &= \frac{1}{e^x} \left[\int e^x\cdot \left(\cos x - \sin x \right) \cdot dx \right]
\end{align}

Notice also that $\frac{d}{dx}\cos x = -\sin x$ \newline 

And therefore 
\begin{align}
\int e^x\cdot \left[\cos x -\sin x \right]\cdot dx &= e^x\cdot \cos x + C \\ 
\because \int e^x\cdot \left(f(x) + f'(x) \right)\cdot dx &= e^x \cdot f(x) + C  \\
\therefore e^x\cdot y &= e^x\cdot \cos x + C  \\
\implies y &= \cos x + \frac{C}{e^x} 
\end{align}

\end{document}