\documentclass[14pt,fleqn]{extarticle}
\RequirePackage{prepwell-eng}

\previewoff

\begin{document} 

\begin{snippet}
    
    
    \incorrect

\[ \lim_{x\to 1} \dfrac{x^2-3x+2}{x^2+3x-4} = \infty\]
    
    \reason

\begin{align}
\dfrac{x^2-3x+2}{x^2 + 3x- 4} &= \dfrac{(x-1)\cdot (x-2)}{(x-1)\cdot (x+4)} \\ 
&= \dfrac{x-2}{x+4} \\ 
\therefore \lim_{x\to 1} \dfrac{x^2-3x+2}{x^2+3x-4} &= \lim_{x\to 1}\dfrac{x-2}{x+4} \\ 
&= \dfrac{\lim_{x\to 1} (x-2)}{\lim_{x\to 1}(x+4)} \\
&= -\dfrac{1}{5}
\end{align}
    
\end{snippet} 
\end{document} 