\documentclass[14pt,fleqn]{extarticle}
\RequirePackage{prepwell}

\newcommand\lx{\lambda x}
\newcommand\ly{\lambda y} 

\previewoff 

\begin{document} 
\begin{snippet}
    \correct
    
    $F(x,y) = \dfrac{x^2 + y^2}{x-y}$ is a homogenous function of degree 1
    
    \reason
    
    \begin{align}
    F(x,y) &= \dfrac{x^2 + y^2}{x-y} \\
    \therefore F \left(\lx,\ly \right) &= \dfrac{ \left(\lx \right)^2 + \left(\ly \right)^2}{\lx - \ly} \\
    &= \lambda\cdot\dfrac{x^2 + y^2}{x-y} \\
    &= \lambda^1\cdot F(x,y) 
\end{align}

Hence, we can see that as $\lambda^n = \lambda^1$, therefore $n=1\implies$ degree $=1$
    
\end{snippet} 
\end{document} 