
\ifnumequal{\value{rolldice}}{0}{
  \renewcommand\va{6}
}{
  \ifnumequal{\value{rolldice}}{1}{
    \renewcommand\va{3}
  }{
    \ifnumequal{\value{rolldice}}{2}{
      \renewcommand\va{4}
    }{
      \renewcommand\va{5}
    }
  }
}

\SUBTRACT\va{1}\vb
\SQUARE\va\vc


\question[2] Differentiate the following with respect to $x$
\[ f(x) = \int_{x^\va}^1 \ln z\ud z \] 

\watchout

\begin{solution}[\halfpage]
  Let $z=e^y$ so that 
  \begin{align}
    \ln z &= \ln e^y = y \text{ and } dz = e^y\cdot dy \\
    \implies\int \ln z\cdot dz &= \int y\cdot e^y\cdot dy
  \end{align}

  Now, if 
  \begin{align}
    g(y) &= y \text{ and } h(y) = e^y\implies h'(y) = e^y 
  \end{align} 

  then the last integral boils down to 
  \begin{align}
    \int y\cdot e^y dy &= \int g(y)\cdot h'(y)\cdot dy \\
    &= \underbrace{g(y)\cdot h(y)-\int g'(y)\cdot h(y)\cdot dy}_{\text{integration by parts}} \\
    &= y\cdot e^y - \int\dfrac{d}{dy}y\cdot e^y\cdot dy = y\cdot e^y - e^y + C \\
    &= \ln z\cdot z - z + C 
  \end{align} 

  Hence, 
  \begin{align}
    f(x) = \int_{x^\va}^1 \ln z\cdot dz &= \left[ z\cdot\ln z - z \right]_{x^\va}^1 
    = \overbrace{x^\va - x^\va\cdot\va \ln x - 1}^{\ln x^a = a\ln x} \\
    \implies \dfrac{d}{dx}f(x) &= \va x^\vb - \va\cdot\underbrace{\left( \dfrac{x^\va}{x} - \va\cdot x^\vb\cdot\ln x \right)}_{\text{Chain Rule}} \\
    &= \vc x^\vb\cdot\ln x
  \end{align}
\end{solution}

\ifprintanswers\begin{codex}$\vc x^\vb\cdot\ln x$\end{codex}\fi
