

\ifnumodd{\value{rolldice}}{
  \renewcommand\va{3}
  \renewcommand\vb{1}
  \renewcommand\vc{\sqrt{3}}
  \renewcommand\vd{ }
  \renewcommand\vx{\sqrt{3}}
  \renewcommand\vy{1}
  \renewcommand\vz{6}
}{
  \renewcommand\va{1}
  \renewcommand\vb{3}
  \renewcommand\vc{ }
  \renewcommand\vd{\sqrt{3}}
  \renewcommand\vx{1}
  \renewcommand\vy{\sqrt{3}}
  \renewcommand\vz{3}
}

%\ifnumequal{\value{rolldice}}{0}{
%}{
%  \ifnumequal{\value{rolldice}}{1}{
%    \renewcommand\va{1}
%    \renewcommand\vb{3}
%    \renewcommand\vc{}
%  }{
%    \ifnumequal{\value{rolldice}}{2}{
%      \renewcommand\va{1}
%      \renewcommand\vb{1}
%      \renewcommand\vc{}
%    }{
%      \renewcommand\va{3}
%      \renewcommand\vb{1}
%      \renewcommand\vc{}
%    }
%  }
%}

\question[4] What are the values of $A$ and $B$ if 
  \[ \int(\vc\sin x - \vd\cos x)\ud x = A\cos\left(x-B\right) + C \]
Hint: $\cos (x-y) = \eCosOfDiff{x}{y}$

\watchout

\begin{solution}[\halfpage]
  \begin{align}
    \int (\vc\sin x - \vd\cos x) \ud x &= -\vc\cos x - \vd\sin x + C \\
    &= \underbrace{-2\cdot\left( \dfrac{\vc\cos x}{\sqrt{\va + \vb}} + \dfrac{\vd\sin x}{\sqrt{\va + \vb}} \right)}
    _{\text{Multiply and divide by }\sqrt{1^2+\sqrt{3}^2}}+ C  \\
    &= -2\cdot\left(\dfrac\vx{2}\cdot\cos x + \dfrac\vy{2}\cdot\sin x \right) + C 
  \end{align}

  \textbf{Insight \#1: $\cos\frac\pi\vz=\frac\vx{2}$ and $\sin\frac\pi\vz=\frac\vy{2}$}

  Which means, 
  \begin{align}
    -2\cdot\left(\dfrac\vx{2}\cdot\cos x + \dfrac\vy{2}\cdot\sin x \right) &= 
    -2\cdot\left( \cos\frac\pi\vz\cos x + \sin\frac\pi\vz\sin x \right) \\
    &= -2\cos\left( x - \frac\pi\vz \right) 
  \end{align}
  And hence, 
  \[ \int (\vc\sin x - \vd\cos x) \ud x = -2\cos\left( x - \frac\pi\vz \right) + C \implies A = -2\text{ and } B = \dfrac\pi\vz \]
\end{solution}

\ifprintanswers\begin{codex}$A=-2\text{ and } B = \dfrac\pi\vz$\end{codex}\fi
