\documentclass[14pt,fleqn]{extarticle}
\RequirePackage{prepwell-eng}

\newcommand\fx{ \left(1 + \log x \right)}
\newcommand\fy{ \left(1-y^2 \right)}
\newcommand\elogx{\left(e^{\log x} \right)} 

\previewoff 

\begin{document} 
\begin{problem}
	\statement 
    
    Find the particular solution of the differential equation 
    \[ \fy\fx\cdot dx + 2xy\cdot dy = 0\]
    given that $ y = 0$ when $x = 1$           
    
    \begin{step}
  \begin{options} 
     \correct 
      
     Given below are \underline{two possible strategies}
     \begin{center}
  \begin{tabular}{NN}
   \toprule
        & \text{Re-write as}  \\
   \midrule
   A & \underbrace{\left(\frac{1}{x^2}-\frac{y^2}{x^2} \right)\fx dx + 2\frac{y}{x} dy = 0}_{\text{Solve as a homogenous differential equation}} \\ 
    \midrule 
    B & \underbrace{-\frac{2y}{\fy}dy = \frac{\fx}{x}dx}_{\text{Solve by separating variables}}\\
    \bottomrule
  \end{tabular}
\end{center}

Of these, only \underline{Strategy $B$ is valid}
       
     \incorrect
     
     Given below are \underline{two possible strategies}
     \begin{center}
  \begin{tabular}{NN}
   \toprule
        & \text{Re-write as}  \\
   \midrule
   A & \underbrace{\left(\frac{1}{x^2}-\frac{y^2}{x^2} \right)\fx dx + 2\frac{y}{x} dy = 0}_{\text{Solve as a homogenous differential equation}} \\ 
    \midrule 
    B & \underbrace{-\frac{2y}{\fy}dy = \frac{\fx}{x}dx}_{\text{Solve by separating variables}}\\
    \bottomrule
  \end{tabular}
\end{center}

Of these, only \underline{Strategy $A$ is valid}
        
    \end{options} 
     \reason 
     
     \begin{align}
	\fy&\fx dx + 2xy\cdot dy = 0 \\[-50pt]
	\implies\dydx &= \frac{-2xy}{\fy\cdot\fx} \\[5pt]
	&= \underbrace{-\dfrac{2\frac{y}{x}}{\left(\frac{1}{x^2}-\frac{y^2}{x^2} \right)\fx}}_{\text{Divide throughtout by }x^2} \\[5pt]
	&\neq F \left(\frac{y}{x} \right)
\end{align}

Hence, Strategy $A$ \underline{is not valid}. However 
\begin{align}
-2xy\cdot dx &= \fy\cdot\fx\cdot dx \\[-20pt]
\text{or } \frac{-2y}{\fy}\cdot dy &= \frac{\fx}{x}\cdot dx 
\end{align}

The variables have separated cleanly. And hence, Strategy $B$ suggests a way forward
       
\end{step}

\begin{step}
  \begin{options} 
     \correct 
       
     If $w = \fx$ and $z = \fy$, then
     \begin{align}
     \int \frac{dz}{z} &= \int w\cdot dw \\
     \therefore \log z &= \frac{w^2}{2} + C \\
     \implies \fy^2 &= k\cdot e^{\fx^2}
\end{align}
     \incorrect
     
     If $w = \fx$ and $z = \fy$, then
     \begin{align}
     \int \frac{dz}{z} &= \int \frac{dw}{w}\\
     \therefore \log z &= \log w + C  \\
     \implies \frac{\fy}{\fx} &= k 
\end{align}
        
    \end{options} 
     \reason 
       
     \begin{align}
     w = \fx &\implies dw = \frac{dx}{x} \\
     z = \fy &\implies dz = -2y\cdot dy\\[5pt]
     \therefore \frac{-2y}{\fy}\cdot dy &= \frac{\fx}{x}\cdot dx \\
     \implies \frac{dz}{z} &= w\cdot dw \\
     \text{or }\int \frac{dz}{z} &= \int w\cdot dw \\
     \implies \log z &= \frac{w^2}{2} + C_1 \\
     \text{or } 2\log z &= \log z^2 = w^2 + C \\
     \implies z^2 &= e^{w^2 + C} \\
     &= e^C\cdot e^{w^2} = k\cdot e^{w^2}\\[10pt]
     \therefore \fy^2 &= k\cdot e^{\fx^2} 
\end{align}  
\end{step}

\begin{step}
  \begin{options} 
     \correct 
     
     \begin{align}
     k\cdot e^{\fx^2} &= k\cdot e\cdot x^2\cdot x^{\log x} \\
     \therefore \fy^2 &= k_2\cdot x^{ \left(\log x + 2 \right)}
\end{align}
        
    \end{options} 
     \reason 
       
     \begin{align}
     k\cdot e^{\fx^2} &= k\cdot e^{\left(1+2\log x + \left(\log x \right)^2 \right)} \\
     &= k\cdot \left[ e^1\cdot e^{2\log x}\cdot e^{\log x\cdot \log x}\right] \\[-10pt]
     &= \underbrace{k\cdot \left[e^1\cdot \elogx^2\cdot \elogx^{\log x} \right]}_{a^{bc} = \left(a^b \right)^c} \\[-10pt]
     &= \underbrace{k_2 \cdot \left(x\right)^2\cdot \left(x \right)^{\log x}}_{e^{\log x} = x} \\[10pt]
     &= k_2\cdot x^{\left( \log x + 2\right)}
\end{align}  

And hence, the \underline{final answer} is
\[\qquad\qquad \fy^2 = k_2 \cdot x^{\left(\log x + 2 \right)}\]
\end{step}
\end{problem} 
\end{document} 