


\ifnumequal{\value{rolldice}}{0}{
  % variables 
  \renewcommand{\va}{2} %p
  \renewcommand{\vb}{3} %q
  \renewcommand\vj{2}
  \renewcommand\vk{3}
  \renewcommand\vu{sum of first $n-2+1=n-1$ odd numbers}
}{
	\ifnumequal{\value{rolldice}}{1}{
		\renewcommand{\va}{3}
    \renewcommand{\vb}{7}
    \renewcommand\vj{2}
    \renewcommand\vk{4}
    \renewcommand\vu{sum of first $n-2+1=n-1$ odd numbers}
	}{
	  \ifnumequal{\value{rolldice}}{2}{
      \renewcommand{\va}{2}
      \renewcommand{\vb}{5}
      \renewcommand\vj{2}
      \renewcommand\vk{3}
      \renewcommand\vu{sum of first $n-2+1=n-1$ odd numbers}
	  }{
      \renewcommand{\va}{3}
      \renewcommand{\vb}{5}
      \renewcommand\vj{2}
      \renewcommand\vk{4}
      \renewcommand\vu{sum of first $n-2+1=n-1$ odd numbers}
	  }
	}
}

\EXPR[0]\af{1-\va + \vb}
\EXPR[0]\as{4-(2*\va)+\vb}
\EXPR[0]\at{9-(3*\va)+\vb}
\EXPR[0]\afo{16-(4*\va)+\vb}

\EXPR[0]\tp{3 * \va}
\EXPR[0]\tq{6 * \vb}
\EXPR[0]\tr{3 * (\va - 1)}
\EXPR[0]\ts{\tq - \tp + 1}

\SUBTRACT\as\af\df
\SUBTRACT\at\as\ds
\SUBTRACT\afo\at\dt

\question[4] Evaluate the expression for the sum of the first $n$ terms of the 
series 
\[ \af + \as + \at + \afo \ldots \]

\watchout

\begin{solution}[\halfpage]
  Before we can calculate $S_n=\sum a_n$, we need an expression for $a_n$. 

  Note that
  \begin{align}
    a_2 - a_1 &= \as-\af=\df \\
    a_3 - a_2 &= \at-\as=\ds \\
    a_4-a_3 &= \afo-\at = \dt \\
    a_n - a_{n-1} &= \vj n - \vk,\, n > 1 \\
  \end{align}

  If we \textbf{add the differences}, then we get 
  \begin{align}
    \sum_{k=2}^n (a_k - a_{k-1}) &= (a_n-a_{n-1}) + (a_{n-1}-a_{n-2}) + \ldots + (a_3-a_2) + (a_2-a_1)  \\
     &= a_n-a_1 = \sum_{k=2}^n (\vj k - \vk) \\
     \implies a_n &= \af + \vj\sum_{k=2}^n k -\vk\sum_{k=2}^n 1 \\
                  &= \af + 2\left[ \dfrac{n\cdot (n+1)}{2} - 1\right] - \vk\cdot( n - 1) \\
                  &= n^2-\va n + \vb
  \end{align}
  
  And therefore,
	\begin{align}
		S_n &= \sum_{k=1}^{n}a_k = \sum_{k=1}^{n}\lbrace k^2 - \va k + \vb \rbrace \\
		&= \sum_{k=1}^{n}k^2 - \va\cdot\sum_{k=1}^{n}k + \vb\cdot\sum_{k=1}^{n}1 \\
		&= \eSumOfSquares{n} - \va\cdot\eSumOfN{n} + \vb\cdot n \\
    &= \dfrac{n}{6}\lbrace (n+1)\cdot(2n+1) - \tp\cdot(n+1) + \tq \rbrace \\
    &= \dfrac{n}{6}\left[ \lbrace (n+1)\cdot(2n + 1 - \tp)\rbrace + \tq \right] \\
    &= \dfrac{n}{6}\left( 2n^2 - \tr n + \ts \right)
	\end{align}
\end{solution}
\ifprintanswers
  \begin{codex}
    $\dfrac{n}{6}\left( 2n^2 - \tr n + \ts \right)$
  \end{codex}
\fi
