
\question[4] Without using a calculator, find the value of 
\[ A = \sin^4\dfrac{\pi}{8} + \sin^4\dfrac{3\pi}{8} + \sin^4\dfrac{5\pi}{8} + \sin^4\dfrac{7\pi}{8} \]

\begin{solution}[\fullpage]
    \textbf{Insight \#1}
    \begin{align}
      \dfrac{7\pi}{8} &= \pi-\dfrac\pi{8} \implies\sin\dfrac{7\pi}{8}=\sin\left(\pi-\dfrac\pi{8} \right) = \sin\dfrac\pi{8} \\
      \dfrac{5\pi}{8} &= \pi-\dfrac{3\pi}{8} \implies\sin\dfrac{5\pi}{8}=\sin\left(\pi-\dfrac{3\pi}{8} \right) = \sin\dfrac{3\pi}{8}
    \end{align}

    Hence, the original expression can be re-written as 
    \begin{align}
      A &= 2\cdot\left[ \sin^4\dfrac\pi{8} + \sin^4\dfrac{3\pi}{8} \right] 
    \end{align}
    \textbf{Insight \#2}
    \[ \dfrac{3\pi}{8} = \dfrac\pi{2} - \dfrac\pi{8} \implies \sin\dfrac{3\pi}{8} = \sin\left(\dfrac\pi{2}-\dfrac\pi{8} \right) = \cos\dfrac\pi{8} \]
    And therefore
    \begin{align}
      A &= 2\cdot\left[ \sin^4\dfrac\pi{8} + \sin^4\dfrac{3\pi}{8} \right] 
         = 2\cdot\left[ \sin^4\dfrac\pi{8} + \cos^4\dfrac{\pi}{8} \right]  \\
        &= 2\cdot\overbrace{\left[ \left(\sin^2\dfrac\pi{8}+\cos^2\dfrac\pi{8}\right)^2 
           - 2\sin^2\dfrac\pi{8}\cdot\cos^2\dfrac\pi{8}\right]}^{a^2+b^2=(a+b)^2-2ab} \\
        &= 2\cdot\left[ 1 - 2\sin^2\dfrac\pi{8}\cdot\cos^2\dfrac\pi{8}\right]
    \end{align}
    \textbf{Insight \#3}
    \[ \dfrac\pi{4} = 2\cdot\dfrac\pi{8} \] 

    \begin{align}
        A  &= 2\cdot\left[ 1 - 2\sin^2\dfrac\pi{8}\cdot\cos^2\dfrac\pi{8}\right] \\
           &= 2\cdot\left[1 - 2\cdot\dfrac{1-\cos\frac\pi{4}}{2}\cdot\dfrac{1+\cos\frac\pi{4}}{2} \right] \\
           &= 2\cdot\left[ 1-\dfrac{1}{2}\cdot\left( 1+\dfrac{1}{\sqrt{2}} \right)\cdot\left( 1-\dfrac{1}{\sqrt{2}} \right) \right] = \dfrac{3}{2}
    \end{align}
\end{solution}

\ifprintanswers\begin{codex}$\dfrac{3}{2}$\end{codex}\fi
