\documentclass[14pt,fleqn]{extarticle}
\RequirePackage{prepwell}
\previewoff
\begin{document}

%text
Find the equation of the tangent to the 
curve $x = \sin 3t, y = \cos 2t$ at $t = \frac\pi{4}$
%

\newcard

%text
The required tangent will touch the curve at 
the point $A = \left(\frac{1}{\sqrt{2}},0 \right)$
%

\newcard

%text
The required tangent will touch the curve at points 
$\underbrace{A = \left(\frac{1}{\sqrt{2}},0 \right)}_{t = \frac\pi{4}} \text{ and } \underbrace{B = \left(0,1\right)}_{t = 0}$
%

\newcard

%text
What we have here is a \underline{parametric curve}
where both $x$ and $y$ are defined in terms 
of the parameter $t$\newline 

As the required line is a tangent, it 
will touch the curve at \underline{only one point} given by
\[ \qquad A = \underbrace{\left(\sin\frac{3\pi}{4}, \cos\frac{2\pi}{4} \right)}_{t=\frac\pi{4}} = \left(\frac{1}{\sqrt{2}}, 0 \right)\]

%

\newcard

%text
The slope $m$ of the required tangent is

\[ \qquad m = \left[\dfrac{dy}{dx}\right]_{t=\frac\pi{4}} = \frac{2\sqrt{2}}{3}\]


\newcard

%text
The slope $m$ of the required tangent is 

\[ \qquad m = \left[\dfrac{dy}{dx}\right]_{t=\frac\pi{4}} = -\frac{2\sqrt{2}}{3}\]
%

\newcard

%text
The slope $m$ will be as follows  

%
\begin{align}
m &= \left[\frac{dy}{dx}\right]_{t=\frac\pi{4}} = \left[\frac{dy / dt}{dx / dt}\right]_{t=\frac\pi{4}} \\
&= \left[\dfrac{-2\sin 2t}{3\cos 3t}\right]_{t=\frac\pi{4}} = \dfrac{-2\times 1}{3\times -\frac{1}{\sqrt{2}}} \\
&= \frac{2\sqrt{2}}{3} 
\end{align}

\newcard

%text
The tangent is therefore 
\[\frac{y - 0}{x - \frac{1}{\sqrt{2}}} = \frac{2\sqrt{2}}{3}
\implies 3y = 2\sqrt{2} x -2 \]


\newcard

%text
The tangent is therefore 
\[ \frac{y-\frac{1}{\sqrt{2}}}{x-0} = \frac{2\sqrt{2}}{3}\implies 3\sqrt{2} y = 4x + 3 \]

%

\newcard

%text
We know the slope of the tangent $(m)$
and the one point it passes through $A$\newline

Hence, the equation is simply 

\begin{align}
\dfrac{y - y_A}{x - x_A} &= m \implies \dfrac{y - 0}{\left( x-\frac{1}{\sqrt{2}}\right)} = \dfrac{2\sqrt{2}}{3} \\
\text{or } 3y &= 2\sqrt{2}\cdot\left( x - \frac{1}{\sqrt{2}}\right) = 2\sqrt{2}x - 2 
\end{align}

\end{document}