

\question[3] If the following equation is true, find $M$.
  \[\dfrac{3\tan\theta-\tan^3\theta}{1-3\tan^2\theta}=\tan M\theta\]

\begin{solution}[\halfpage]
  Expand the Left Hand Side (L.H.S) of the equation,
  \begin{align}
		\text{L.H.S} &= \dfrac{3\tan\theta-\tan^3\theta}
				           {1-3\tan^2\theta} \\
                 &= \dfrac{\tan\theta(1-\tan^2\theta)+2\tan\theta}
                          {1-\tan^2\theta-2\tan^2\theta} \\
                 &\small{\textit{Multiply and divide by }
                   (1-\tan^2\theta)}\nonumber \\
                 &= \dfrac{\tan\theta+\dfrac{2\tan\theta}{1-\tan^2\theta}}
                          {\left(1-\dfrac{2\tan^2\theta}
                                         {1-\tan^2\theta}\right)} \\
                 &\small{\textit{Using $\tan(A+B)$ expansion for 
                   $\tan 2\theta$}}\nonumber \\
                 &= \dfrac{\tan\theta+\tan 2\theta}
                          {1-\tan 2\theta\tan\theta} \\
                 &= \tan(\theta+2\theta) = \tan 3\theta
  \end{align}
  Therefore, $M=3$

\end{solution}
\ifprintanswers\begin{codex}$M=3$\end{codex}\fi
