


\ifnumequal{\value{rolldice}}{0}{
  % variables 
  \renewcommand{\va}{2} %p
  \renewcommand{\vb}{1} %p
  \renewcommand\vz{\dfrac{n}{3}\cdot(4n^2+6n-1)}
}{
	\ifnumequal{\value{rolldice}}{1}{
		\renewcommand{\va}{3}
    \renewcommand{\vb}{1} %p
    \renewcommand\vz{\dfrac{n}{2}\cdot(6n^2+9n+1)}
	}{
	  \ifnumequal{\value{rolldice}}{2}{
      \renewcommand{\va}{3}
      \renewcommand{\vb}{2} %p
      \renewcommand\vz{\dfrac{n}{2}\cdot(6n^2+9n-5)}
	  }{
      \renewcommand{\va}{2}
      \renewcommand{\vb}{3} %p
      \renewcommand\vz{\dfrac{n}{3}\cdot(4n^2+6n-25)}
	  }
	}
}

\SQUARE\va\vc
\SQUARE\vb\vd
\MULTIPLY\vc{2}\ve

\EXPR[0]\a{\vc-\vd}
\EXPR[0]\b{4*\vc-\vd}
\EXPR[0]\c{9*\vc-\vd}
\EXPR[0]\d{16*\vc-\vd}

\SUBTRACT\b\a\w
\SUBTRACT\c\b\x
\SUBTRACT\d\c\y

\SUBTRACT\ve\vc\vj
\SUBTRACT\vj\a\vk

\question[3] Find an expression for the sum of the first $n$ terms of the series 
  \[ \a + \b + \c + \d + \ldots \] 

\watchout

\begin{solution}[\halfpage]
  \textbf{Step \#1: Finding an expression for $a_n$ - the $n-$th term}
  
  If we see the series as 
  \[ S = a_1 + a_2 + a_3 + a_4 + \ldots \]
  then notice that 
  \begin{align}
    a_2 - a_1 &= \w = \vc\cdot (1+2) \\
    a_3 - a_2 &= \x = \vc\cdot (3+2) \\
    a_4 - a_3 &= \y = \vc\cdot (4+3) \\
    \implies a_n - a_{n-1} &= \vc\cdot (n + n-1) = \vc\cdot (2n-1)
  \end{align}
  And therefore, 
  \[ \underbrace{(a_n-a_{n-1}) + (a_{n-1}-a_{n-2}) + \ldots + (a_2-a_1)}_{\text{middle terms cancel out}}
   = a_n-a_1 \]
   \begin{align}
      a_n - a_1 &= \sum_{k=2}^n (\ve n - \vc) = 
      \left[ \sum_{k=1}^n(\ve n - \vc) - \underbrace{(8-4)}_{k=1}\right] \\
      &= \ve\sum_{k=1}^n n - \vc\sum_{k=1}^n 1 - \vj \\
      \implies a_n &= \left[\ve\eSumOfN{n} - \vc n \right] - (\vj-\a) 
      = \underbrace{(\vc n^2 - \vd)}_{\text{on simplification}}
   \end{align}

  \textbf{Step \#2: Add up the $a_n$} 

  \begin{align}
    S &= \sum_{k=1}^n a_n = \sum_{k=1}^n (\vc n^2 - \vd) 
      = \vc \sum_{k=1}^n n^2 - \vd\sum_{k=1}^n 1 \\
      &= \vc\eSumOfSquares{n} - \vd n = \vz
  \end{align}
\end{solution}

\ifprintanswers\begin{codex}$\vz$\end{codex}\fi
