\documentclass[14pt,fleqn]{extarticle}
\RequirePackage{prepwell}
\previewoff

\newcommand\tsqx{\tan^2\frac{x}{2}}
\newcommand\tsqy{\tan^2 \frac{y}{2}}
\newcommand\ea{\frac{a-b}{a+b}}


\begin{document}

\begin{question}
	\statement 
    
     Prove the following 
     \small\[ 2\tan^{-1} \left(\sqrt{\ea}\cdot\tan \frac{x}{2} \right) = \cos^{-1} \left(\frac{a\cos x + b}{a + b\cos x} \right)\] \normalsize
     
     \begin{step}
  \begin{options} 
     \correct 
       
       Because 
       \small\[ y = 2\tan^{-1} \left(\sqrt{\ea}\cdot\tan \frac{x}{2} \right) = \cos^{-1} \left(\frac{a\cos x + b}{a + b\cos x} \right)\] \normalsize
       
       Therefore 
       \begin{align}
	\tan \frac{y}{2} &= \sqrt{\ea}\cdot\tan \frac{x}{2} \\
	\text{and } \cos y &= \frac{a\cos x + b}{a + b\cos x}
\end{align}

\incorrect
 
Because 
       \small\[ y = 2\tan^{-1} \left(\sqrt{\ea}\cdot\tan \frac{x}{2} \right) = \cos^{-1} \left(\frac{a\cos x + b}{a + b\cos x} \right)\] \normalsize

Therefore 
\[ \tan \frac{y}{2} = \sqrt\ea\cdot\tan \frac{x}{2} = \cos y = \frac{a\cos x + b}{a + b\cos x}\]       
        
    \end{options} 
     \reason 
     
     This problem looks scarier than it is. So, let us do the simplest things first 
     
     \small\[ y = 2\tan^{-1} \left(\sqrt{\ea}\cdot\tan \frac{x}{2} \right) = \cos^{-1} \left(\frac{a\cos x + b}{a + b\cos x} \right)\] \normalsize
     
     And hence 
     \begin{align}
     y &= 2\tan^{-1} \left(\sqrt{\ea}\cdot\tan \frac{x}{2} \right) \\
     \frac{y}{2} &= \tan^{-1} \left(\sqrt\ea\cdot\tan \frac{x}{2} \right) \\
     \text{or } \tan \frac{x}{2} &= \sqrt\ea\cdot\tan\frac{x}{2}
\end{align}

Similarly 
\begin{align}
y &= \cos^{-1} \left( \frac{a\cos x + b}{a + b\cos x}\right) \\
	\therefore \cos y &= \frac{a\cos x + b}{a + b\cos x}
\end{align}
       
This \underline{does not} mean that $\tan \frac{y}{2} = \cos y$ (just in case you 
were wondering) 

\end{step}

\begin{step}
  \begin{options} 
     \correct 
     
     \begin{align}
	\cos y &= \frac{1 - \tsqy}{1 + \tsqy} \\
	&= \left[ \frac{1-\ea\cdot\tsqx}{1 + \ea\cdot\tsqx}\right] \\
	&= \left[\frac{a\cdot \left(1-\tsqx \right) + b\cdot \left(1+\tsqx \right)}{a\cdot \left(1+\tsqx \right) + b\cdot \left(1-\tsqx \right)} \right] \\
	&= \frac{a\cdot\cos x + b}{a + b\cdot \cos x}\quad\text{ (hence proved)}
\end{align}

        
    \end{options} 
     \reason 

     We know that 
     \[ \qquad \cos 2\theta = \frac{1-\tan^2\theta}{1+\tan^2\theta}\]
     
     Similarly, 
     
     \begin{align}
	\cos y &= \frac{1 - \tsqy}{1 + \tsqy} \\
	&= \left[ \frac{1-\ea\cdot\tsqx}{1 + \ea\cdot\tsqx}\right] \\
	&= \left[\frac{a+b-a\tsqx + b\tsqx}{a+b+a\tsqx - b\tsqx} \right] \\
	&= \left[\frac{a\cdot \left(1-\tsqx \right) + b\cdot \left(1+\tsqx \right)}{a\cdot \left(1+\tsqx \right) + b\cdot \left(1-\tsqx \right)} \right] \\
	&= \left[\underbrace{\frac{a\cdot \left( \frac{1-\tsqx}{1+\tsqx}\right) + b}{a + b\cdot \left(\frac{1-\tsqx}{1+\tsqx}\right)}}_{\text{Noticed }\cos x?} \right] \\
	&= \frac{a\cdot\cos x + b}{a + b\cdot \cos x}\quad\text{ (hence proved)}
\end{align}
       
\end{step}
\end{question} 

\end{document}