

\question[3] Find an expression for the sum of the first $n$ terms of the following series
\[ \dfrac{1}{1\cdot 4} + \dfrac{1}{4\cdot 7} + \ldots + \dfrac{1}{(3n-2)\cdot(3n+1)} + \ldots \]

\begin{solution}[\halfpage]
  If $a_k$ be the $k-$th term of the series, then 
  \begin{align}
     a_k &= \dfrac{1}{(3k-2)\cdot (3k+1)} = \dfrac{1}{3}\cdot\dfrac{(3k+1)-(3k-2)}{(3k-2)\cdot(3k+1)} \\
     & = \dfrac{1}{3}\cdot\left[ \dfrac{1}{3k-2}-\dfrac{1}{3k+1} \right] \\
		\implies S_n &= \sum_{k=1}^n a_k = \dfrac{1}{3}\left[ \sum_{k=1}^{n}\dfrac{1}{3k-2} - \sum_{k=1}^{n}\dfrac{1}{3k+1}\right] \\
		    &= \dfrac{1}{3}\cdot\left[\underbrace{\left( 1+\frac{1}{4}+\ldots +\frac{1}{3n-2}\right)
		    - \left( \frac{1}{4} + \ldots + \frac{1}{3n-2} + \frac{1}{3n+1}\right)}_{\text{middle terms cancel out}} \right] \\
		    &= \dfrac{1}{3}\cdot\left( 1-\dfrac{1}{3n+1}\right) = \dfrac{n}{3n+1}
	\end{align}
\end{solution}
\ifprintanswers\begin{codex}$\dfrac{n}{3n+1}$\end{codex}\fi
