
\question[5] Evaluate the following integral 
\[ I = \int\sin^6 x\ud x \]
Think standard trigonometric results.

\begin{solution}[\fullpage]
  \textbf{Insight \#1: $\sin^2\theta = \dfrac{1-\cos 2\theta}{2}$}
  
  \begin{align}
    I &= \int\sin^6 x\ud x = \int(\sin^2 x)^3\ud x \\
    &= \int\left[\dfrac{1-\cos 2x}{2} \right]^3\ud x = \dfrac{1}{8}\cdot\int (1-\cos 2x)^3\ud x \\
    &= \dfrac{1}{8}\cdot\int\underbrace{(1-3\cos 2x + 3\cos^2 2x - \cos^3 2x)}_{(a-b)^3 = a^3 - 3a^2b + 3ab^2 - b^3}\ud x \\
    &= \dfrac{1}{8}\cdot\left[\int\ud x - 3\int\cos 2x\ud x + \underbrace{3\cdot\int\cos^2 2x\ud x}_{A} - \underbrace{\int\cos^3 2x\ud x}_{B} \right] \\
    &= \dfrac{1}{8}\cdot\left[ x -\dfrac{3}{2}\sin 2x + A - B \right]
  \end{align}
  \textbf{Insight \#2: $\cos^2\theta = \dfrac{1+\cos 2\theta}{2}$}

  \begin{align}
    A &= 3\cdot\int\cos^2 2x\ud x = \dfrac{3}{2}\cdot\int(1+\cos 4x)\ud x \\
      &= \dfrac{3}{2}\cdot\left[ \int\ud x + \int\cos 4x\ud x \right] \\
      &= \dfrac{3}{2}\cdot\left( x + \dfrac{\sin 4x}{4} \right) + C_A
  \end{align} 
  \textbf{Evaluating $B$}

  \begin{align}
    B &= \int\cos^3 2x\ud x = \int\underbrace{(1-\sin^2 2x)}_{=\cos^2 2x}\cdot\cos 2x\ud x
  \end{align}
  Now, if we let $z = \sin 2x$, then 
  \[ \ud z = 2\cdot\cos 2x\ud x \implies \cos 2x\ud x = \dfrac{\ud z}{2} \]
  Which means, 
  \begin{align}
    B &= \int(1-\sin^2 2x)\cos 2x\ud x = \dfrac{1}{2}\cdot\int (1-z^2)\ud z \\
     &= \dfrac{1}{2}\cdot\left[ \int\ud z - \int z^2\ud z \right] \\
     & = \dfrac{z}{2}\left( 1 - \dfrac{z^2}{3} \right) + C_B \\
     & = \dfrac{\sin 2x}{2}\cdot\left( 1-\dfrac{\sin^2 2x}{3}\right) + C_B 
  \end{align}
  \textbf{Putting it all together}

  And hence, 
  \begin{align}
    I &= \dfrac{1}{8}\cdot\left[ x -\dfrac{3}{2}\sin 2x + A - B \right] \\
      &= \dfrac{1}{8}\cdot\left[ x - \dfrac{3}{2}\sin 2x + 
         \dfrac{3}{2}\cdot\left( x + \dfrac{\sin 4x}{4} \right) - 
         \dfrac{\sin 2x}{2}\cdot\left( 1-\dfrac{\sin^2 2x}{3}\right)\right] \\
      &= \dfrac{1}{8}\cdot\left[\dfrac{5}{2}x - 2\sin 2x + \dfrac{3}{8}\sin 4x + \dfrac{\sin^3 2x}{6} \right] + C 
  \end{align}
\end{solution}

\ifprintanswers
  \begin{codex}
    $\dfrac{1}{8}\cdot\left[\dfrac{5}{2}x - 2\sin 2x + \dfrac{3}{8}\sin 4x + \dfrac{\sin^3 2x}{6} \right] + C$
  \end{codex}
\fi
