\documentclass[14pt,fleqn]{extarticle}
\RequirePackage{prepwell-eng}
\previewoff

\newcommand\fx{\alpha\sin 2t\cdot \left(1+\cos 2t \right)}
\newcommand\fy{\beta\cos 2t\cdot \left(1-\cos 2t \right)}

\begin{document}

\begin{problem}
	\statement 
    
     Find $\dfrac{dy}{dx}$ if $x = \fx$ and $y=\fy$       
     
   \begin{step}
  \begin{options} 
     \correct 
       \[ \qquad x' = 4\alpha\cdot\cos 3t\cdot \cos t \]
     \incorrect
        \[ \qquad x' = 2\alpha\cdot\cos 2t\cdot \cos t \]
    \end{options} 
     \reason 
     
     This is a \underline{parametric curve} in which both $x$ and $y$ are defined 
     in terms of a third parameter $t$. Which is why
     
     \begin{align}
	 x &= \fx \\
	 \therefore \frac{dx}{dt} &= \underbrace{\alpha \left[\left(1+\cos 2t \right)\cdot \left(2\cos 2t \right) - 2\sin^2 2t  \right]}_{\text{Product and Chain Rules}} \\
	 &= \alpha \left[2\cos 2t + 2 \underbrace{\left(\cos^2 2t - \sin^2 2t \right)}_{\cos 2\theta = \cos^2\theta - \sin^2\theta} \right] \\
	 &= \underbrace{2\alpha \left(\cos 2t + \cos 4t \right)}_{\cos A + \cos B = 2\cos \frac{A+B}{2}\cdot \cos\frac{B-A}{2}} \\
	 &= 4\alpha\cdot\cos 3t\cdot \cos t
\end{align}
       
\end{step}

\begin{step}
  \begin{options} 
     \correct 
       \begin{align}
	\frac{dy}{dt} &= 4\beta \cdot\cos 3t \cdot \sin t \\
	\therefore \dydx &= \frac{\beta}{\alpha}\tan t
\end{align}
     \incorrect
        
        \begin{align}
	\frac{dy}{dt} &= 4\beta \cdot\sin 3t \cdot \cos t \\
	\therefore \dydx &= \frac{\beta}{\alpha}\tan 3t
\end{align}

    \end{options} 
     \reason 
       
       \begin{align}
	y &= \fy \\
	\therefore \frac{dy}{dt} &= \beta \left[\cos 2t \left(2\sin 2t \right) - 2 \left(1-\cos 2t \right)\sin 2t \right] \\
	&= 2\beta \left[2\sin 2t\cos 2t - \sin 2t  \right] \\
	&= \underbrace{2\beta \cdot \left(\sin 4t - \sin 2t \right)}_{2\sin x\cdot\cos x = \sin 2x } \\
	&= \underbrace{2\beta\cdot \left(2\cos 3t\cdot\sin t \right)}_{\sin A - \sin B = 2\cos \frac{A+B}{2}\cdot \sin \frac{A-B}{2}} \\
	&= 4\beta \cdot\cos 3t \cdot \sin t 
\end{align}

Hence \[ \dydx = \frac{dy / dt}{dx / dt} = \frac{4\beta \cdot\cos 3t \cdot \sin t}{4\alpha\cdot\cos 3t\cdot \cos t} = \frac{\beta}{\alpha}\tan t\]
\end{step}
\end{problem} 
\end{document}