\documentclass[14pt,fleqn]{extarticle}
\RequirePackage{prepwell}

\previewoff 

\begin{document} 
\begin{snippet}
    \correct
    
    The integrating factor of the following differential equation is $\dfrac{1}{x}$
    \[\qquad\quad x\dydx - y = x^4 - 3x \]

    
    \reason
    
    \begin{align}
	x\dydx - y &= x^4 - 3x \implies \dydx - \frac{y}{x} = x^3 - 3 
\end{align}

This looks like $\dfrac{dy}{dx} +P(x)\cdot y = Q(x)$ where $P(x) = -\dfrac{1}{x}$ \newline 

And hence, the integrating factor is 
\begin{align}
I &= e^{\int P(x)\cdot dx} = e^{\int -\frac{dx}{x}} \\
&= \underbrace{e^{-\log x} = \frac{1}{e^{\log x}} = \frac{1}{x}}_{a^{-b} = \frac{1}{a^b}\text{ and } e^{\log a} = a}
\end{align}
    
\end{snippet} 
\end{document} 