
\documentclass[14pt,fleqn]{extarticle}
\RequirePackage{prepwell-eng}
\previewoff

\newcommand\dnm{\sin^2x\cdot \cos^2x} 
\newcommand\fx{\frac{\sin^6 + \cos^6 x}\dnm}

\begin{document}
\begin{problem}
	\statement 
    
     Evaluate the following integral 
     \[ \quad I = \int \fx \cdot dx \] 
     
     \begin{step}
  \begin{options} 
     \correct 
      
      \begin{align}
	I &= \int\fx\cdot dx \\
	&= \underbrace{\int \frac{\sin^6 x}{\dnm}\cdot dx}_P + \underbrace{\int \frac{\cos^6 x}{\dnm}\cdot dx}_Q 
\end{align}

\begin{center}
  \begin{tabular}{NN}
   \toprule
       \text{Integral} & \text{Equals} \\
   \midrule 
   P & \int \left(\sec^2 x + \cos^2 x - 2 \right) dx \\ 
    \midrule
    Q & \int \left(\csc^2 x + \sin^2 x -2 \right)dx \\  
    \bottomrule
  \end{tabular}
\end{center}

        
    \end{options} 
     \reason 
     
Generally speaking, $\int \left[ f(x) + g(x)\right] \cdot dx$ is easier to 
evaluate than $\int f(x)\cdot g(x)\cdot dx$ or $\int \frac{f(x)}{g(x)}\cdot dx$ \newline 

 Hence, try the simpler option out first

\begin{align}
	I &= \int \fx \cdot dx \\
	&= \underbrace{\int \frac{\sin^6 x}{\dnm}\cdot dx}_P  \\
	&+ \underbrace{\int \frac{\cos^6 x}{\dnm}\cdot dx }_Q  \\
	P &= \int \frac{\sin^4 x}{\cos^2 x}\cdot dx = \int \frac{\left(1-\cos^2x \right)^2}{\cos^2 x}\cdot dx \\
	&= \int \frac{\cos^4 x + 1 - 2\cos^2 x}{\cos^2 x}\cdot dx \\
	&= \int \left(\sec^2 x + \cos^2 x - 2 \right)\cdot dx \\
	Q &= \int \frac{\cos^4 x}{\sin^2 x}\cdot dx = \int \frac{\left(1-\sin^2 x \right)^2}{\sin^2 x}\cdot dx \\
	&= \int \frac{\sin^4 x + 1 - 2\sin^2 x}{\sin^2 x}\cdot dx \\ 
	&= \int \left(\sin^2 x + \csc^2 x - 2 \right)\cdot dx 
\end{align}
\end{step}

\begin{step}
  \begin{options} 
     \correct 
     
     \begin{align}
	I &= P + Q = \int \left(\sec^2 x + \csc^2 x - 3 \right)\cdot dx \\
	&= \tan x + \cot x -3x + C 
\end{align}
       
    \end{options} 
     \reason 
     
     Simply adding the two integrals $P$ and $Q$ back together again to get $I$
     \begin{align}
	I &= P + Q \\ 
	&= \int \left(\sec^2 x + \cos^2 x - 2 \right)\cdot dx \\
	&+ \int \left(\csc^2 x + \sin^2 x - 2 \right)\cdot dx \\ 
	&= \int \left(\sec^2 + \csc^2 \right) dx + \int \underbrace{\left(\sin^2x + \cos^2 x\right)}_{=1} dx \\
	&- 2\int dx - 2\int dx \\
	&= \int \left(\sec^2 x + \csc^2 x \right)dx + \int dx - 4 \int dx \\
	&= \int \left(\sec^2 x + \csc^2 x - 3\right)\cdot dx 
\end{align}
       
\end{step}

\begin{step}
  \begin{options} 
     \correct 
       
       \[ I = \tan x - \cot x - 3x + C \]
     \incorrect
        
         \[ I = \tan x\cdot \sec x +\cot x - 3x + C \]
    \end{options} 
     \reason 
       
       \begin{align}
	I &= \int \left(\sec^2x + \csc^2 x - 3 \right)\cdot dx \\ 
	&= \int \sec^2 x\cdot dx + \int \csc^2 x \cdot dx - 3 \int dx \\
	&= \tan x - \cot x - 3x + C 
\end{align}
\end{step}
\end{problem} 
\end{document}