\documentclass[14pt,fleqn]{extarticle}
\RequirePackage{prepwell}

\newcommand\itanx{\tan^{-1} x}
\newcommand\itany{\tan^{-1} y}

\newcommand\trma{\left(1+x^2 \right)}
\newcommand\trmb{ \left(1+y^2 \right)}

\previewoff 

\begin{document} 
\begin{snippet}
    \correct
    
    $\itanx + \itany = c$ is the general solution of 
    \[ \qquad \left(1+x^2 \right)\cdot dy + \left(1+y^2 \right)\cdot dx = 0 \]    
    
    \reason
    
    If $\itanx + \itany = c$, then 
    \begin{align}
	&\ddx \itanx + \ddx \itany = \underbrace{\ddx c = 0}_{\ddx\text{constant} = 0}\\
	&\implies \frac{1}{1+x^2} + \underbrace{\frac{1}{1+y^2}\cdot \dydx}_{\text{Chain Rule}} = 0 \\
	&\text{or }\frac{1}{1+y^2}\cdot \dydx = -\frac{1}{1+x^2} \\
	&\text{or }\trma\cdot dy = -\trmb\cdot dx \\
	&\text{or }\trma\cdot dy + \trmb\cdot dx = 0 
\end{align}

In other words, if 
\[\quad \trma\cdot dy + \trmb\cdot dx = 0\] is the differential equation, then  
\[ \quad \itanx + \itany = c\]
is the general solution
    
\end{snippet} 
\end{document} 