\documentclass[14pt,fleqn]{extarticle}
\RequirePackage{prepwell-eng}

\newcommand\nmr{\sqrt{x}-1}
\newcommand\dnm{\sqrt{x}+1}

\previewoff 

\begin{document} 
\begin{snippet}
    \correct
    
    If $y = \sec^{-1} \left(\dfrac\dnm\nmr \right) + \sin^{-1} \left(\dfrac\nmr\dnm \right)$ then $\dfrac{dy}{dx} = 0$ 
    
    \reason
    
    This looks a lot more complicated than it is \newline 
    
    \begin{align}
	 &\sec^{-1} \left(\frac\dnm\nmr \right) + \sin^{-1} \left(\frac\nmr\dnm\right) \\
	 &= \underbrace{\cos^{-1} \left(\frac\nmr\dnm \right) + \sin^{-1} \left(\frac\nmr\dnm \right)}_{\sec^{-1} x = \cos^{-1} \frac{1}{x}} \\
	 &= \frac\pi{2} \quad (\because \cos^{-1}\theta + \sin^{-1}\theta = \frac\pi{2}) 
\end{align}
   
   Hence, $ y = \dfrac\pi{2}\implies \dfrac{dy}{dx}  = 0$
\end{snippet} 
\end{document} 