\documentclass[14pt,fleqn]{extarticle}
\RequirePackage{prepwell}
\previewoff
\begin{document}

\newcommand\dnm{5-4e^x-e^{2x}}
\newcommand\zply{5-4z-z^2}
\newcommand\psqr{9- \left(z +2 \right)^2}

%text
Evaluate the following integral \[ \qquad I = \int \frac{e^x}{\sqrt{\dnm}}\cdot dx \]
%

\newcard

If $z = e^x$, then 
\begin{align}
I &= \int \frac{dz}{\sqrt{\zply}} = \int \frac{dz}{\sqrt{\psqr}}
\end{align}

\newcard 

If $z = e^x$, then 
\begin{align}
I &= \int \frac{z\cdot dz}{\sqrt{\zply}} = \int \frac{dz}{\sqrt{6- \left(z+2 \right)^2}}
\end{align}

\newcard 

\begin{align}
	\text{If } z &= e^x \text{ then } dz = e^x\cdot dx \\
	\text{and } \underbrace{\dnm}_{ e^{2x} = \left(e^x \right)^2 = z^2} &= \zply  \\
	&= 5 - \left[\left(z+2 \right)^2 - 4\right] \\
	&= 5 - \left(z+2 \right)^2 + 4 \\
	&= 9 - \left(z+2 \right)^2
\end{align}

\newcard 

\[ I = \int \frac{dz}{\sqrt{\psqr}} = \sin^{-1} \left(\frac{e^x+2}{3} \right) + C\]

\newcard 

\begin{align}
I &= \int \frac{dz}{\sqrt{\psqr}} = \int \frac{dz}{\sqrt{3^2 - \left(z+2 \right)^2}} \\ 
&= \sin^{-1} \left(\frac{z+2}{3} \right) + C = \sin^{-1} \left(\frac{e^x + 2}{3} \right) + C 
\end{align}

We have used the standard result 
\[ \qquad \int \frac{dx}{\sqrt{a^2 - x^2}} = \sin^{-1} \left(\frac{x}{a} \right) + C \] 
\end{document}