\documentclass[14pt,fleqn]{extarticle}
\RequirePackage{prepwell}

\previewoff

\begin{document}

\begin{snippet}
    \correct

\[\int_0^1\cot^{-1}\left(\dfrac{1}{1-x} \right)\cdot dx = \int_0^1\tan^{-1} x\cdot dx \]
    
    
    \reason

\begin{align}
	\cot^{-1} \dfrac{1}{z} &= \tan^{-1} z \\
	\therefore \cot^{-1} \left(\frac{1}{1-x} \right) &= \tan^{-1} \left(1-x \right) \\
	\implies \int_0^1 \cot^{-1} \left(\frac{1}{1-x} \right)\cdot dx &= \int_0^1 \tan^{-1} \left(1-x \right)\cdot dx 
\end{align}
	
But recall that
 
\begin{align} 
	\int_0^a f(x)\cdot dx &= \int_0^a f(a-x)\cdot dx  \\
	\therefore\int_0^1 \tan^{-1} \left(1-x \right)\cdot dx &= \int_0^1\tan^{-1} \left[1-\left(1-x \right) \right]\cdot dx \\
	&=\int_0^1\tan^{-1} x\cdot dx  
\end{align}
    
\end{snippet} 

\end{document}
