
\question Given the series 
\[ 1 + \dfrac{1}{1+2} + \dfrac{1}{1+2+3} + \dfrac{1}{1+2+3+4}\ldots \]

\begin{parts}
  \part[3] Find an expression for the sum of the first $n$ terms

\begin{solution}[\halfpage]
  	\begin{align}
  		S_n &= 1 + \dfrac{1}{1+2} + \dfrac{1}{\underbrace{1+2+3}_{\text{Sum of first $k$ integers}}} + \dfrac{1}{1+2+3+4}\ldots \\
  		&= \sum_{k=1}^{n}\dfrac{1}{\eSumOfN{k}} = 2\cdot\sum_{k=1}^{n}\dfrac{1}{k\cdot(k+1)} \\
  		&= 2\cdot\sum_{k=1}^{n}\dfrac{k+1-k}{k\cdot(k+1)} \\
  		&= 2\cdot\left[ \sum_{k=1}^{n}\dfrac{1}{k} - \sum_{k=1}^{n}\dfrac{1}{k+1} \right] \\
  		&= 2\cdot\left[ 1 + \underbrace{\sum_{k=2}^{n}\dfrac{1}{k} - \sum_{k=1}^{n-1}\dfrac{1}{k+1}}
  		_{\text{= 0. Convinced?}}- \dfrac{1}{n+1}\right] \\
  		&= \dfrac{2n}{n+1}
  	\end{align}
  \end{solution}

  \part[1] The sum of the series if $n=\infty$ 

\begin{solution}[\mcq]
  \begin{align}
    S_n &= \dfrac{2n}{n+1} = \dfrac{2}{1+\frac{1}{n}} \\
    \implies S_\infty &= \dfrac{2}{1+0} = 2
  \end{align}
\end{solution}

\end{parts}
\ifprintanswers
  \begin{codex}
    \begin{tabular}{c c}
      $(a)\quad\dfrac{2n}{n+1}$ & $(b)\, 2$
    \end{tabular} 
  \end{codex}
\fi
