\documentclass[14pt,fleqn]{extarticle}
\RequirePackage{prepwell}

\newcommand\fx{\pi\sin \left(\pi x \right) + 2x - 4}
\newcommand\expb{ \left(x-2 \right)^2 + 2\sin^2 \left(\frac{\pi x}{2} \right)}

\previewoff 

\begin{document} 
\begin{question}
	\statement 
    
    For what values of $x$ does the anti-derivative of $f(x) = \fx$ which has the value $3$ when $x = 1$ vanish? 
    
    \begin{step}
  \begin{options} 
     \correct 
       
       We have to find $x$ for which 
       \[ \, F(x) = \int \left[\fx \right]\cdot dx = 0  \]
     \incorrect
     
     We have to find $x$ for which 
       \[ \quad f(x) = \fx = 0 \]
        
    \end{options} 
     \reason 
     
     It is the anti-derivative of $f(x)$ that has to vanish. Which means we have to find the $x$'s where 
     \[ \qquad F(x) = \int f(x)\cdot dx = 0 \]
     
     given that $F(1) = 3$ 
       
\end{step} 

\begin{step}
  \begin{options} 
     \correct 
       
       If $F(1) = 3$ then 
       \[\quad F(x) = -\cos \left(\pi x \right) + x^2 - 4x + 5 \]
       
     \incorrect
        
        If $F(1) = 3$ then 
       \[\quad F(x) = -\cos \left(\pi x \right) + x^2 - 4x + 7 \]
    \end{options} 
     \reason 
       
       \begin{align}
	F(x) &= \int f(x)\cdot dx \\
	&= \int \left[\fx \right]\cdot dx \\
	&= \left[\pi\cdot\frac{-\cos \left(\pi x \right)}{\pi} + 2\cdot\frac{x^2}{2} - 4x\right] + C \\
	&= -\cos \left(\pi x \right)+ x^2 - 4x + C
\end{align}

But $F(1) = 3$. And therefore 
\begin{align}
F(1) = 3 &\implies -\cos \pi + 1^2 - 4 + C = 3 	\\
\text{or } 3 &= 1 + 1 -4 + C \implies C = 5 
\end{align}
\end{step}

\begin{step}
  \begin{options} 
     \correct 
       \begin{align}
	F(x) &= -\cos \left(\pi x \right) + x^2 - 4x + 5 \\
	&= \left(x-2 \right)^2 + 2\sin^2 \left(\frac{\pi x}{2} \right)
\end{align}

\incorrect 

 \begin{align}
	F(x) &= -\cos \left(\pi x \right) + x^2 - 4x + 5 \\
	&= \left(x-1 \right)^2 + 2\cos^2 \left(\frac{\pi x}{2} \right)
\end{align}
        
    \end{options} 
     \reason 
       
       \begin{align}
       F(x) &=  -\cos \left(\pi x \right) + \overbrace{x^2 - 4x + 5}^{A} \\
       &= \underbrace{\left(x^2-4x+4 \right) + 1}_{A} -\cos \left(\pi x \right) \\
       &= \left(x-2 \right)^2 + \left[1-\cos \left(\pi x \right) \right] \\
       &= \left(x-2 \right)^2 + \underbrace{2\sin^2 \left(\frac{\pi x}{2} \right)}_{1-\cos 2\theta = 2\sin^2\theta}
\end{align}
\end{step}

\begin{step}
  \begin{options} 
       
     \incorrect 
     
     If $F(x) = \expb = 0$ then 
     \[ \qquad \left(x-2 \right)^2 = - 2\sin^2 \left(\frac{\pi x}{2} \right)\]
       
     But this can't happen for any value of $x$. Hence, \underline{there is no valid value of $x$} 
    
    \end{options} 

 \reason
     
     If $F(x) = \expb$ then 
     \[ \qquad F(x) = 0 \implies \begin{cases} 
     \left(x-2 \right)^2 = 0 \\
     2\sin^2 \left(\frac{\pi x}{2} \right) = 0
     \end{cases} \]
     This is possible \underline{only if $x = 2$} as at $x=2, \left(x-2 \right)=0$ and $\sin \left(\frac{\pi x}{2} \right) = \sin \pi x = 0$ 
       
\end{step}
\end{question} 
\end{document} 