

\printrubric

\question[4] Find an expression for the sum of the first $n$ terms of the series 
\[ \dfrac{1}{1\cdot 2\cdot 3} + \dfrac{1}{2\cdot 3\cdot 4} + \dfrac{1}{3\cdot 4\cdot 5} + \ldots \]

\begin{solution}[\fullpage]
	Each term in the series is of the form $a_n = \dfrac{1}{n\cdot(n+1)\cdot(n+2)}$. And therefore,
	\begin{align}
		S_n &= \sum_{k=1}^{n}\dfrac{1}{k\cdot(k+1)\cdot(k+2)} 
		= \sum_{k=1}^{n}\dfrac{k+1-k}{k\cdot(k+1)\cdot(k+2)} \\
		&= \sum_{k=1}^{n}\dfrac{1}{k\cdot(k+2)} - \sum_{k=1}^{n}\dfrac{1}{(k+1)\cdot(k+2)} \\
		&= \dfrac{1}{2}\sum_{k=1}^{n}\dfrac{k+2-k}{(k+2)\cdot k} - \sum_{k=1}^{n}\dfrac{k+2-(k+1)}{(k+1)\cdot(k+2)} \\
		&= \dfrac{1}{2}\underbrace{\left[\sum_{k=1}^{n}\dfrac{1}{k} - \sum_{k=1}^{n}\dfrac{1}{k+2} \right]}_{A}
		- \underbrace{\left[ \sum_{k=1}^{n}\dfrac{1}{k+1} - \sum_{k=1}^{n}\dfrac{1}{k+2} \right]}_{B} \\
		&= \dfrac{1}{2}A - B
  \end{align}
	Now, 
	\begin{align}
		A &= \underbrace{\left[\left(1 + \frac{1}{2} + \frac{1}{3} + \ldots + \frac{1}{n} \right) 
		- \left( \frac{1}{3} + \frac{1}{4} + \ldots + \frac{1}{n} + \frac{1}{n+1} + \frac{1}{n+2}\right) 
		\right]}_{\text{middle terms cancel out}} \\
		&= \left( 1+\dfrac{1}{2}\right) - \left( \dfrac{1}{n+1} + \dfrac{1}{n+2}\right) = 
		\dfrac{3}{2}-\dfrac{1}{n+1}-\dfrac{1}{n+2} \\
		&= \dfrac{3n^2 + 5n}{4\cdot(n+1)\cdot(n+2)}
  \end{align}
	As for $B$,
	\begin{align}
		B &= \underbrace{\left[ \left(\dfrac{1}{2}+\dfrac{1}{3} + \ldots + \dfrac{1}{n+1} \right) - 
		\left( \dfrac{1}{3} + \dfrac{1}{4} + \ldots + \dfrac{1}{n+1} + \dfrac{1}{n+2} \right) \right]}
		_{\text{middle terms cancel out}} \\
		&= \dfrac{1}{2}-\dfrac{1}{n+2} = \dfrac{n}{2\cdot(n+2)}
	\end{align}
	And therefore, 
	\begin{align}
		S_n &= \dfrac{1}{2}A - B = \dfrac{3n^2 + 5n}{4\cdot(n+1)\cdot(n+2)} - \dfrac{n}{2\cdot(n+2)} \\
		&= \dfrac{n\cdot (n+3)}{4\cdot (n+1)\cdot (n+2)}
	\end{align}
\end{solution}

\ifprintanswers\begin{codex}$\dfrac{n\cdot (n+3)}{4\cdot (n+1)\cdot (n+2)}$\end{codex}\fi
