\documentclass[14pt,fleqn]{extarticle}
\RequirePackage{prepwell}

\previewoff

\begin{document}

\begin{skill}
\begin{narrow}
\textcolor{blue}{Inverse Trigonometry (Reciprocals)}

\small{\textbf{Example} }$\quad \sin^{-1}\dfrac{1}{x} = \csc^{-1} x$
\end{narrow}

\reason 

%text
We will prove one result, namely
\[ \qquad \sin^{-1}\frac{1}{x} = \csc^{-1} x\]
$\ldots$ and then perhaps you can try and prove the other results given below

%
\begin{align}
\csc\theta &= x \implies \frac{1}{\sin\theta} =x \\
\therefore \sin\theta &= \frac{1}{x} 
\implies \theta = \sin^{-1}\frac{1}{x} \\
\text{But }\theta &= \csc^{-1} x \\
\therefore \csc^{-1}x &= \sin^{-1}\frac{1}{x} 
\end{align}
%text

Similarly 
%
\begin{align}
\sec^{-1} x &= \cos^{-1}\frac{1}{x} \\ 
\cot^{-1} x &= \tan^{-1}\frac{1}{x} \quad (x >  0) \\
&= -\pi + \cot^{-1} x \quad (x < 0) 
\end{align}

\end{skill}
\end{document}
