\documentclass[14pt,fleqn]{extarticle}
\RequirePackage{prepwell-eng}

\previewoff

\begin{document}
\begin{snippet}
    \correct
    
\[ \int_1^2 x^2\cdot dx = \int_1^2 (3-x)^2\cdot dx \]    

    \reason

Recall the following standard result 
\[ \quad \int_a^b f(x)\cdot dx = \int_a^b f(a+b-x)\cdot dx \]

When applied to $\int_1^2 x^2\cdot dx$, one can see that 
\begin{align}
	\int_1^2 x^2\cdot dx &= \int_1^2 \left(1+2-x \right)^2\cdot dx  \\
	&= \int_1^2 \left(3-x \right)^2\cdot dx 
\end{align}
    
\end{snippet} 
\end{document}
