\documentclass[14pt,fleqn]{extarticle}
\RequirePackage{prepwell-eng}
\previewoff

\newcommand\logx{\log\vert x\vert}

\begin{document}
\begin{problem}
\statement
	
%text
Find the particular solution, satisfying the 
given condition, for the following differential
equation
\[ \quad\frac{dy}{dx} -\frac{y}{x} + \csc\frac{y}{x} = 0 ; y = 0\text{ when }  x = 1 \] 
Note: $\csc =$ cosec
%
\begin{step}
	\begin{options}
		\correct

\[ \qquad \frac{dy}{dx} = \underbrace{\frac{y}{x} - \csc\frac{y}{x}}_{F(x,y)}\]
And as $F \left(\lambda x,\lambda y \right) = F(x,y)$, therefore the given equation is a homogenous differential equation 

		\incorrect

\[ \qquad \frac{dy}{dx} - \frac{1}{x}y =  - \csc\frac{y}{x} \]

The above is of the form 
\[ \qquad \frac{dy}{dx} + P(x)\cdot\frac{dy}{dx} = Q(x) \]
Hence, this is a \underline{linear differential equation}

	\end{options}
	\reason
	
	When written as follows
	\[ \qquad \dydx - \frac{1}{x}y = \underbrace{-\csc\frac{y}{x}}_{Q} \]
	the given differential equation \underline{may look like} a 
	first-order linear differential equation\newline 
	
	But if it is to be a linear differential equation, then $Q = f(x)$ only - which it is not \newline 
	
Instead, $Q = \csc\frac{y}{x} = g \left(x,y \right)$ -  a function of both $x$ and $y$ \newline 

However, when written as 
\[ \qquad \dydx = \frac{y}{x} - \csc\frac{y}{x} = F \left(x,y \right)\]
it becomes clear that what we have is a \underline{homogenous} differential equation
\end{step}
\begin{step}
	\begin{options}
		\correct
		
		If $ y = vx$, then 
		\[\qquad \frac{dx}{x} = -\sin v\cdot dv\]

		\incorrect
		
		If $ y = vx$, then 
		\[\qquad \frac{dv}{dx} - v = -\csc v\]

	\end{options}
	\reason

If we let $\dfrac{y}{x} = v$, then 
	\begin{align}
y = v\cdot x \implies \frac{dy}{dx} &= v + x\cdot\frac{dv}{dx} \\
\therefore \frac{dy}{dx} - \frac{y}{x} &= -\csc\frac{y}{x}\\[5pt]
\implies \left(v+x \frac{dv}{dx}\right) -v &= -\csc v \\
\text{or } x\frac{dv}{dx} &= -\csc v \\[10pt]
\implies \frac{dx}{x} &= -\sin v\cdot dv 
\end{align} 
\end{step}

\begin{step}
	\begin{options}
		\correct
		
		And therefore, 
		\begin{align}
	\logx &= \cos v + C \text{ where } C = -1 \\
	\implies y &= x\cdot\cos^{-1} \left(\logx + 1 \right)
\end{align}
		\incorrect
		
		And therefore, 
		\begin{align}
	\logx &= \cos v + C \text{ where } C = 0 \\
	\implies y &= x\cdot \cos^{-1} \left(\logx \right)
\end{align}

	\end{options}
	\reason

	\begin{align}
\frac{dx}{x} &= -\sin v\cdot dv \\
\implies \int\frac{dx}{x} &= \int -\sin v\cdot dv \\
\therefore \logx  &= \cos v + C \\
 \text{or } \log\vert x\vert &= \cos\frac{y}{x} + C \\
\text{Now } y = 0 & \text{ when }  x = 1 \\
\therefore \log \vert 1\vert &= \cos 0 + C \\
\implies 0 &= 1 + C \text{ or } C = -1\\
\therefore \log\vert x\vert &= \cos\frac{y}{x} - 1\\
\text{or } y &= x\cdot\cos^{-1}\left(\log\vert x\vert + 1 \right) 
\end{align} 
\end{step}
\end{problem}
\end{document}
