\documentclass[14pt,fleqn]{extarticle}
\RequirePackage{prepwell-eng}

\previewoff 

\begin{document} 
\begin{snippet}
    \correct
    
    If $f(x) = \vert \cos x - \sin x\vert$ then 
    \[ \quad f' \left(\frac{\pi}{3} \right) = \left[\sin x + \cos x \right]_{x = \frac{\pi}{3}} = \frac{\sqrt{3}+1}{2} \]
    
    \reason
    
    For $x > \frac\pi{4}, \sin x > \cos x$. Which is why 
    \[ \quad f(x) = \begin{cases} 
    \cos x - \sin x, x \in \left(0, \frac\pi{4} \right) \\
    \sin x - \cos x, x \in \left(\frac\pi{4}, \frac\pi{2} \right)
    \end{cases} \]
    
    And hence, at $x = \frac{\pi}{3}$ 
    \begin{align}
	f'(x) &= \ddx \left(\sin x-\cos x \right) = \cos x + \sin x\\
	\text{or } f' \left(\frac\pi{3} \right) &= \frac{\sqrt{3} + 1}{2}
\end{align}
    
\end{snippet} 
\end{document} 