

\question[4] Find an expression for the sum of the first $n$ terms of the series
\[ 1\cdot 2\cdot 4 + 2\cdot 3\cdot 7 + 3\cdot 4 \cdot 10 + \ldots \] 

\begin{solution}[\halfpage]
  If $a_n$ be the $n-$th term, then note that 
  \[ a_n = n\cdot (n+1) \cdot (3n + 1),\,n\geq 1 \] 
  And hence, the sum of the first $n$ terms would be 
	\begin{align}
		S_n &= \sum_{k=1}^{n}n\cdot(n+1)\cdot(3n+1) = \sum_{k=1}^{n}(3n^3 + 4n^2 + n) \\
		&= 3\cdot\sum_{k=1}^{n}n^3 + 4\cdot\sum_{k=1}^{n}n^2 + \sum_{k=1}^{n}n \\
		&= 3\cdot\eSumOfCubes{n} + 4\cdot\eSumOfSquares{n} + \eSumOfN{n} \\
		&= \dfrac{n\cdot(n+1)}{12}\cdot\left[ 9n\cdot(n+1) + 8\cdot(2n+1) + 6\right] \\
		&= \dfrac{n\cdot(n+1)}{12}\cdot(9n^2 + 25n + 14)
	\end{align}
\end{solution}
\ifprintanswers
  \begin{codex}
	  $\dfrac{n\cdot(n+1)}{12}\cdot(9n^2 + 25n + 14)$
  \end{codex}
\fi
