\documentclass[14pt,fleqn]{extarticle}
\RequirePackage{prepwell}
\previewoff
\begin{document}

\newcommand\xma{\left(x-a \right)}
\newcommand\xpa{\left(x+a \right)}
\newcommand\pma{ \left(\phi-2a \right)}

%text
Evaluate the following integral 
\[ \qquad I = \int \frac{\sin \xma}{\sin \xpa}\cdot dx \]
%

\newcard

\begin{align}
	\text{If } \phi &= \xpa \text{ then } \\
	\frac{\sin\xma}{\sin \xpa} &= \cos 2a - \sin 2a\cdot \frac{\cos\phi}{\sin\phi}
\end{align}

\newcard 

You might be tempted to expand $\sin\xma$ and $\sin \xpa$ \newline 

Try that. But you will find that the resulting expression is not any easier to work with.  Perhaps, a little creativity is required 

\begin{align}
	\text{If } \phi = \xpa &\text{ then } \xma = \phi - 2a \\
	\therefore \frac{\sin\xma}{\sin\xpa} &= \frac{\sin\pma}{\sin\phi} \\
	&= \frac{\sin\phi\cdot\cos 2a + \cos\phi\cdot\sin 2a}{\sin\phi} \\
	&= \cos 2a + \sin 2a\cdot \frac{\cos\phi}{\sin\phi}
\end{align} 

\newcard 

\[ I = \cos 2a\cdot\xpa + \sin 2a\cdot \log \sin \xpa + C \]

\newcard 

\[ I = \cos 2a\cdot\xpa + \frac{\sin 2a}{\sin^2\xpa} + C \]

\newcard 

\begin{align}
	I &= \int \frac{\sin\xma}{\sin\xpa}\cdot dx \\
	&= \underbrace{\int \left[\cos 2a + \sin 2a\cdot \frac{\cos\phi}{\sin\phi} \right]\cdot d\phi}_{\text{Note than }d\phi = dx} \\
	&= \cos 2a\int d\phi + \sin 2a\int \frac{\cos\phi}{\sin\phi}\cdot d\phi \\
	&= \cos 2a\cdot \phi + \sin 2a \underbrace{\int \frac{dz}{z}}_{\text{Let }z = \sin\phi} \\
	&= \cos 2a\cdot\phi + \sin 2a\cdot\log \vert z\vert + C \\
	&= \cos 2a\cdot\xpa + \sin 2a\cdot \log \sin \xpa + C 
\end{align}



\end{document}