


\ifnumequal{\value{rolldice}}{0}{
  % variables 
}{
  \ifnumequal{\value{rolldice}}{1}{
    % variables 
  }{
    \ifnumequal{\value{rolldice}}{2}{
      % variables 
    }{
      % variables 
    }
  }
}

\question If $x + \textit{i} y = \dfrac{a+\textit{i} b}{a - \textit{i}b}$ , prove that $x^{2} + y^{2} = 1$ \\ 


\watchout

\ifprintanswers
  % stuff to be shown only in the answer key - like explanatory margin figures
  \begin{marginfigure}
    \figinit{pt}
      \figpt 100:(0,0)
      \figpt 101:(0,0)
    \figdrawbegin{}
      \figdrawline [100,101]
    \figdrawend
    \figvisu{\figBoxA}{}{%
    }
    \centerline{\box\figBoxA}
  \end{marginfigure}
\fi 

\begin{solution}
Rationalizing the term on the right hand side 
\begin{align}
\Rightarrow \dfrac{a+\textit{i} b}{a - \textit{i}b} &= \dfrac{a+\textit{i} b}{a - \textit{i}b} \times \dfrac{a+\textit{i} b}
{a + \textit{i}b} \\
&= \dfrac{a^2 - b^2 + 2\cdot a \cdot b \textit{i}}{a^2 + b^2} \\	
x + \textit{i}y &= \dfrac{a^2 - b^2}{a^2 + b^2} + \dfrac{2\cdot a \cdot b \textit{i}}{a^2 + b^2} \\
\Rightarrow x &= \dfrac{a^2 - b^2}{a^2 + b^2} \quad \text{and} \quad	
y = \dfrac{2\cdot a \cdot b}{a^2 + b^2} \\
x^2 + y^2 &= \left(\dfrac{a^2 - b^2}{a^2 + b^2}\right)^2 +  \left(\dfrac{2\cdot a \cdot b}{a^2 + b^2}\right)^2	\\
&= \dfrac{({a^2 - b^2})^2 + ({2\cdot a \cdot b})^2}{({a^2 + b^2})^2} 	 \\
&= \dfrac{({a^2 + b^2})^2}{({a^2 + b^2})^2} = 1 
\end{align}
\end{solution}


