\documentclass[14pt,fleqn]{extarticle}
\RequirePackage{prepwell}
\previewoff
\begin{document}

\newcommand\ea{ \left(x^2-1 \right)}
%text
Solve the following differential equation
\[ \quad \ea\frac{dy}{dx} + 2xy = \frac{1}{\ea}, \vert x\vert \neq 1\]
%

\newcard

\[ \ea\frac{dy}{dx} + 2x\cdot y = \frac{1}{\ea}\]
is of the form \[ \qquad \frac{dy}{dx} = F \left(\frac{y}{x} \right)\]
which makes it a \underline{homogenous} differential equation
\newcard 

\begin{align}
	\ea \frac{dy}{dx}+ 2xy &= \frac{1}{\ea} \\
	\implies \frac{dy}{dx} + \frac{2x}{\ea}\cdot y&= \frac{1}{\ea^2}
\end{align}

The above looks like 
\[ \qquad \frac{dy}{dx} + P(x)\cdot y = Q(x) \]

And that we know is a \underline{first-order linear} differential equation -- not a homogenous one 

\newcard 

\[ \ea \frac{dy}{dx} + 2x\cdot y = \frac{d}{dx} \left[\ea\cdot y \right]\]

\newcard 

\[ \ea \frac{dy}{dx} + 2x\cdot y \neq \frac{d}{dx} \left[\ea\cdot y \right]\]

\newcard 

We have established that the given differential equation is a linear one\newline 

And so, the logical next step would be to calculate the integrating factor. It would be \underline{perfectly ok} to do that\newline 

But if you can be a little patient, then you will notice that $\frac{d}{dx}\ea = 2x$\newline  

And furthermore 
\begin{align}
\frac{d}{dx} \left[\ea\cdot y \right] &= \underbrace{\ea \frac{dy}{dx} + y\cdot \frac{d}{dx}\ea}_{\text{Product Rule}} \\
&= \underbrace{\ea\cdot \frac{dy}{dx} + 2x\cdot y}_{\text{Our differential equation!}}
\end{align}

\newcard 

\begin{align}
	\frac{d}{dx} \ea\cdot y &= \frac{1}{\ea^2} \\
	\implies y &= \frac{1}{2\ea} \cdot \log \left\vert \frac{x-1}{x+1}\right\vert + C 
\end{align}

\newcard 

\begin{align}
	\frac{d}{dx} \ea\cdot y &= \frac{1}{\ea^2} \\
	\implies y &= \frac{1}{\ea}\cdot\tan^{-1} x + C 
\end{align} 

\newcard 

In the last step, we established that 
\[ \qquad \frac{d}{dx} \left[\ea\cdot y \right] = \frac{1}{\ea}\]

And so it follows that 

\begin{align}
\ea\cdot y &= \int \frac{dx}{x^2-1} \\
&= \underbrace{\frac{1}{2}\cdot \log \left\vert \frac{x-1}{x+1}\right\vert}_{\text{Standard result}} + C  \\
\implies y &= \frac{1}{2\ea}\log \left\vert \frac{x-1}{x+1}\right\vert + C 
\end{align}
\end{document}