\documentclass[14pt,fleqn]{extarticle}
\RequirePackage{prepwell-eng}

\previewoff 

\begin{document} 
\begin{problem}
	\statement 
    
    Find the value of 
    \[ \qquad y = \sin \left(2\tan^{-1}2 \right)\]
          
    \begin{step}
  \begin{options} 
     \correct 
     
       $\tan^{-1}2$ is an angle. And therefore 
       \[ \quad \phi = \tan^{-1} 2\implies y = \dfrac{2\tan\phi}{1+\tan^2\phi}\]

     \incorrect
        
        $\tan^{-1}2$ is an angle. And therefore 
       \[ \quad \phi = \tan^{-1} 2\implies y = \dfrac{2\tan\phi}{1-\tan^2\phi}\]
    \end{options} 
     \reason 
     
     Yes, $\tan^{-1} 2$ is an angle. And if that angle be $\phi$, then 
     \begin{align}
	y &= \sin \left(2\phi \right) = 2\sin\phi\cdot\cos\phi \\
	&= \dfrac{2\sin\phi\cos\phi}{\underbrace{\sin^2\phi + \cos^2\phi}_{=1}} = \underbrace{\dfrac{2\tan\phi}{1+\tan^2\phi}}_{\text{Divide throughout by }\cos^2\phi}
\end{align}
       
\end{step}

\begin{step}
  \begin{options} 
     \correct 
       
     And hence, $y = \sin \left(2\tan^{-1} 2 \right) = \dfrac{4}{5}$ 
     \incorrect
     
     And hence, $y = \sin \left(2\tan^{-1} 2 \right) = \dfrac{3}{5}$ 
        
    \end{options} 
     \reason 
     
     \begin{align}
     y &= \dfrac{2\tan\phi}{1+\tan^2\phi} \text{ where } \underbrace{\tan\phi = 2}_{\phi = \tan^{-1} 2} \\
     \therefore y &= \dfrac{2\times 2}{1+2^2} = \dfrac{4}{5}  
\end{align}
     
     
       
\end{step}
\end{problem} 
\end{document} 