


\ifnumequal{\value{rolldice}}{0}{
  % variables 
  \renewcommand{\va}{5} 
  \renewcommand{\vd}{4} 
  \renewcommand\vz{\dfrac{n}{3}\cdot (2n^2 + 6n + 7)}
}{
	\ifnumequal{\value{rolldice}}{1}{
		\renewcommand{\va}{4}
    \renewcommand{\vd}{2}
    \renewcommand\vz{\dfrac{n}{3}\cdot (n^2+3n+8)}
	}{
	  \ifnumequal{\value{rolldice}}{2}{
      \renewcommand{\va}{3}
      \renewcommand{\vd}{2}
      \renewcommand\vz{\dfrac{n}{3}\cdot (n^2+3n+5)}
	  }{
      \renewcommand{\va}{6}
      \renewcommand{\vd}{2}
      \renewcommand\vz{\dfrac{n}{3}\cdot (n^2+3n+14)}
	  }
	}
}

\DIVIDE\vd{2}\ve
\SUBTRACT\va\vd\vf % a_n = \ve n^2 + \ve n + \vf 

\EXPR[0]\vi{6*\ve + \vf}
\EXPR[0]\vj{12*\ve + \vf}
\EXPR[0]\vk{20*\ve + \vf}

\question[3] Find an expression for the sum of the first $n$ terms of the series 
\[ \va + \vi + \vj + \vk + \ldots \]

\watchout

\begin{solution}[\halfpage]
  \textbf{Step \#1: Finding an expression for $a_n$ in terms of $n$}

  If we think of the above series as 
  \[ S = a_1 + a_2 + a_3 + a_4 \ldots \]
  then notice that 
  \begin{align}
    a_2 - a_1 &= \vi-\va = \vd\times 2 \\ 
    a_3 - a_2 &= \vj-\vi = \vd\times 3 \\ 
    a_4 - a_3 &= \vk-\vj = \vd\times 4 \\ 
    \implies a_n - a_{n-1} &= \vd\times n
  \end{align}
  Which means, 
  \[ \overbrace{(a_n-a_{n-1}) + (a_{n-1} + a_{n-2})\ldots + (a_2-a_1)}^{\text{middle terms cancel out}} = a_n - a_1 \]
  And therefore, 
  \begin{align}
    a_n - a_1 &= \sum_{k=2}^n \vd k = \vd\cdot\left[ \sum_{k=1}^n k - 1 \right] = 
    \vd\cdot\left[ \dfrac{n\cdot(n+1)}{2} - 1 \right] \\
    \implies a_n &= a_1 + \vd\cdot\left[ \dfrac{n\cdot(n+1)}{2} - 1 \right] = \ve n^2 + \ve n + \vf 
  \end{align}
  \textbf{We can now find the required expression for $\sum_{k=1}^n a_n$}
  \begin{align}
    S_n &= \sum_{k=1}^n a_n = \sum_{k=1}^n (\ve n^2 + \ve n + \vf) \\ 
    &= \ve\cdot\sum_{k=1}^n n^2 + \ve\cdot\sum_{k=1}^n n + \vf\cdot\sum_{k=1}^n 1 \\ 
    &= \ve\cdot\eSumOfSquares{n} + \ve\cdot\eSumOfN{n} + \vf n \\
    &= \underbrace{\vz}_{\text{on simplification}}
  \end{align}
\end{solution}

\ifprintanswers\begin{codex}$\vz$\end{codex}\fi
