

\question[4] If the sum of the first $n$ terms of a series is given by 
$S_n = 2n^2+3n$, then prove that the terms are in arithmetic progression


\ifprintanswers
  % stuff to be shown only in the answer key - like explanatory margin figures
\fi 

\begin{solution}[\halfpage]
  If the terms are in arithmetic progression, then the $(n+1)^{th}$ term should be 
  of the form $k_{n+1} = \underbrace{a}_{\texttt{known}} + n\times\underbrace{d}_{\texttt{known}}$
  
  Moreover,
  \begin{align}
     k_{n+1} &= S_{n+1} - S_n \\
        \Rightarrow k_{n+1} &= 2\cdot(n+1)^2 + 3\cdot(n+1) - 2n^2 - 3n \\
        &= 5 + 4n
  \end{align}
  As $k_{n+1}$ is of the required form, the terms of the series are in arithmetic progression
  
\end{solution}
