\documentclass[14pt,fleqn]{extarticle}
\RequirePackage{prepwell}
\previewoff
\begin{document}

\newcommand\ey{a\cdot \left[\cos t + \log \left(\tan \frac{t}{2} \right) \right]}
%text

If $x=a\sin t$ and $y=\ey$, 
then find $\dfrac{d^2y}{dx^2}$
%

\newcard 

\begin{center}
  \begin{tabular}{NNN}
   \toprule
        \frac{dx}{dt} & \frac{dy}{dt} & \frac{dy}{dx}  \\
   \midrule 
   a\cos t & a\cdot \frac{\cos^2 t}{\sin t} & \cot t  \\
    \bottomrule
  \end{tabular}
\end{center}

\newcard 

What we have here is a \underline{parametric} curve in which both $x$ and $y$ are expressed in terms of a third parameter $t$ \newline 

Moreover, to find $\doublediff$, we will first need to find $\dydx$

\begin{align}
 \frac{dx}{dt} &= \frac{d}{dt} \left(a\cdot\sin t  \right) = a\sin t \\
 \frac{dy}{dt} &= \frac{d}{dt}\left(\ey \right) \\
 &= a \left[-\sin t + \underbrace{\frac{1}{\tan\frac{t}{2}}\cdot\sec^2 \frac{t}{2}\cdot \frac{1}{2}}_{\text{Chain Rule}}  \right] \\
 &= \underbrace{a \left[-\sin t + \frac{1}{2\cdot \frac{\sin \frac{t}{2}}{\cos \frac{t}{2}}\cdot \cos^2 \frac{t}{2}} \right]}_{\sin 2\theta = 2\sin\theta\cdot\cos\theta} \\
 &= a \left[-\sin t + \frac{1}{\sin t} \right] = a \left(\frac{1-\sin^2 t}{\sin t} \right) \\
 &= a\cdot \left(\frac{\cos^2 t}{\sin t} \right) \\
 \therefore \frac{dy}{dx} &= \frac{dy/dt}{dx/dt} = \frac{a\cos^2 t}{a\cos t\cdot \sin t} = \cot t 
\end{align}

\newcard

\begin{align}
	\doublediff &= \frac{d}{dt} \left(\dydx \right)\cdot \frac{dt}{dx} 
\end{align}

\newcard

\begin{align}
	\doublediff &= \frac{d}{dt} \left(\dydx \right)
\end{align}

\newcard 

By definition \[ \qquad \doublediff = \ddx \left(\dydx \right)\]
But if $\dydx = f(t)$, as in this question, then 
\[ \quad \doublediff = \ddx f(t) = \frac{d}{dt} f(t)\cdot \frac{dt}{dx}\]
This is the same as 
\[ \qquad \doublediff = \frac{d}{dt} \left(\dydx \right)\cdot \frac{dt}{dx} \]

\newcard 

\begin{align}
	\doublediff &= -\frac{2}{a\sin t \cdot \sin 2t}
\end{align}

\newcard

\[\doublediff = \dfrac{1}{a\cdot\sin t\cdot \sin 2t} \]

\newcard

\begin{align}
\frac{dy}{dx} &= \cot t \\
\therefore \frac{d^2 y}{dx^2} &= \frac{d}{dt}\cot t\cdot\frac{1}{a\cdot\cos t} = \frac{-\csc^2 t}{a\cdot \cos t} \\
&= \underbrace{-\left[ \frac{2}{a\cdot 2\sin^2 t\cdot\cos t}\right] }_{\text{Multiply and divide by 2}} \\
&= -\dfrac{2}{a\cdot\sin t\cdot (2\sin t\cdot \cos t)} \\ 
&= -\dfrac{2}{a\cdot\sin t\cdot \sin 2t}
\end{align}

\end{document}